# The content of this file is automatically extracted from fip.trig.
# Changes should be made in fip.trig.pre.

@prefix icc: <https://w3id.org/fair/icc/terms/> .
@prefix fair: <https://w3id.org/fair/principles/terms/> .
@prefix rdf: <http://www.w3.org/1999/02/22-rdf-syntax-ns#> .
@prefix owl: <http://www.w3.org/2002/07/owl#> .
@prefix rdfs: <http://www.w3.org/2000/01/rdf-schema#> .
@prefix xsd: <http://www.w3.org/2001/XMLSchema#> .
@prefix dct: <http://purl.org/dc/terms/> .
@prefix pav: <http://purl.org/pav/> .
@prefix prov: <http://www.w3.org/ns/prov#> .
@prefix np: <http://www.nanopub.org/nschema#> .
@prefix npx: <http://purl.org/nanopub/x/> .
@prefix orcid: <https://orcid.org/> .
@prefix foaf: <http://xmlns.com/foaf/0.1/> .

foaf:member a owl:ObjectProperty .
rdfs:seeAlso a owl:ObjectProperty .

fair:FAIR-Principle-or-SubPrinciple rdfs:label "FAIR Principle or Sub-Principle" .

fair:F1 rdfs:label "F1" .
fair:F2 rdfs:label "F2" .
fair:F3 rdfs:label "F3" .
fair:F4 rdfs:label "F4" .
fair:A1.1 rdfs:label "A1.1" .
fair:A1.2 rdfs:label "A1.2" .
fair:A2 rdfs:label "A2" .
fair:I1 rdfs:label "I1" .
fair:I2 rdfs:label "I2" .
fair:I3 rdfs:label "I3" .
fair:R1.1 rdfs:label "R1.1" .
fair:R1.2 rdfs:label "R1.2" .

npx:NanopubIndex rdfs:label "Nanopublication Index" .


<https://w3id.org/fair/fip/terms/FIP-Ontology> a <http://www.w3.org/2002/07/owl#Ontology>;
  <http://purl.org/dc/terms/creator> <https://orcid.org/0000-0001-8888-635X>, <https://orcid.org/0000-0002-1267-0234>,
    <https://orcid.org/0000-0003-2195-3997>;
  <http://purl.org/dc/terms/description> "This is an ontology of the FAIR Implementation Profiles (FIP) for the FAIR principles.";
  <http://purl.org/dc/terms/license> <https://creativecommons.org/publicdomain/zero/1.0/>;
  <http://purl.org/dc/terms/title> "FAIR Implementation Profile (FIP) Ontology";
  <http://purl.org/vocab/vann/preferredNamespacePrefix> "fip";
  <http://purl.org/vocab/vann/preferredNamespaceUri> "https://w3id.org/fair/fip/terms/";
  <http://www.w3.org/2000/01/rdf-schema#isDefinedBy> <https://w3id.org/fair/fip/latest/FIP-Ontology>;
  <http://www.w3.org/2000/01/rdf-schema#seeAlso> <https://w3id.org/fair/principles/terms/FAIR> .

<https://w3id.org/fair/fip/terms/FIP-Question> a <http://www.w3.org/2002/07/owl#Class>;
  <http://www.w3.org/2000/01/rdf-schema#isDefinedBy> <https://w3id.org/fair/fip/latest/FIP-Question>;
  <http://www.w3.org/2000/01/rdf-schema#label> "FIP Question"@en;
  <http://www.w3.org/2004/02/skos/core#definition> "A question communities have to address when declaring their FAIR Implementation Profiles"@en .

<https://w3id.org/fair/fip/terms/FIP-Data-related-Question> a <http://www.w3.org/2002/07/owl#Class>;
  <http://www.w3.org/2000/01/rdf-schema#isDefinedBy> <https://w3id.org/fair/fip/latest/FIP-Data-related-Question>;
  <http://www.w3.org/2000/01/rdf-schema#label> "FIP Data-related Question"@en;
  <http://www.w3.org/2000/01/rdf-schema#subClassOf> <https://w3id.org/fair/fip/terms/FIP-Question>;
  <http://www.w3.org/2004/02/skos/core#definition> "A FIP question that is relevant for the actual data (as compared to just their metadata)"@en .

<https://w3id.org/fair/fip/terms/FIP-Metadata-related-Question> a <http://www.w3.org/2002/07/owl#Class>;
  <http://www.w3.org/2000/01/rdf-schema#isDefinedBy> <https://w3id.org/fair/fip/latest/FIP-Metadata-related-Question>;
  <http://www.w3.org/2000/01/rdf-schema#label> "FIP Metadata-related Question"@en;
  <http://www.w3.org/2000/01/rdf-schema#subClassOf> <https://w3id.org/fair/fip/terms/FIP-Question>;
  <http://www.w3.org/2004/02/skos/core#definition> "A FIP question that is relevant for metadata (as compared to the data themselves)"@en .

<https://w3id.org/fair/fip/terms/FAIR-Declaration> a <http://www.w3.org/2002/07/owl#Class>;
  <http://www.w3.org/2000/01/rdf-schema#isDefinedBy> <https://w3id.org/fair/fip/latest/FAIR-Declaration>;
  <http://www.w3.org/2000/01/rdf-schema#label> "FAIR Declaration"@en;
  <http://www.w3.org/2000/01/rdf-schema#subClassOf> <https://w3id.org/fair/fip/terms/FAIR-Supporting-Resource>;
  <http://www.w3.org/2004/02/skos/core#definition> "The statement of a community on how it addresses a FAIR-related question."@en .

<https://w3id.org/fair/fip/terms/FIP-Declaration> a <http://www.w3.org/2002/07/owl#Class>;
  <http://www.w3.org/2000/01/rdf-schema#isDefinedBy> <https://w3id.org/fair/fip/latest/FIP-Declaration>;
  <http://www.w3.org/2000/01/rdf-schema#label> "FIP Declaration"@en;
  <http://www.w3.org/2000/01/rdf-schema#subClassOf> <https://w3id.org/fair/fip/terms/FAIR-Declaration>;
  <http://www.w3.org/2004/02/skos/core#definition> "The expression of a community on how they address a FIP question"@en .

<https://w3id.org/fair/fip/terms/FSR-Declaration> a <http://www.w3.org/2002/07/owl#Class>;
  <http://www.w3.org/2000/01/rdf-schema#isDefinedBy> <https://w3id.org/fair/fip/latest/FSR-Declaration>;
  <http://www.w3.org/2000/01/rdf-schema#label> "FSR Declaration"@en;
  <http://www.w3.org/2000/01/rdf-schema#subClassOf> <https://w3id.org/fair/fip/terms/FAIR-Declaration>;
  <http://www.w3.org/2004/02/skos/core#definition> "The statement of a community on the usage of a FAIR Supporting Resource."@en .

<https://w3id.org/fair/fip/terms/SIP-Declaration> a <http://www.w3.org/2002/07/owl#Class>;
  <http://www.w3.org/2000/01/rdf-schema#isDefinedBy> <https://w3id.org/fair/fip/latest/SIP-Declaration>;
  <http://www.w3.org/2000/01/rdf-schema#label> "SIP Declaration"@en;
  <http://www.w3.org/2000/01/rdf-schema#subClassOf> <https://w3id.org/fair/fip/terms/FAIR-Declaration>;
  <http://www.w3.org/2004/02/skos/core#definition> "The statement of a community on how it addresses a SIP question."@en .

<https://w3id.org/fair/fip/terms/FAIR-Interpretation> a <http://www.w3.org/2002/07/owl#Class>;
  <http://www.w3.org/2000/01/rdf-schema#isDefinedBy> <https://w3id.org/fair/fip/latest/FAIR-Interpretation>;
  <http://www.w3.org/2000/01/rdf-schema#label> "FAIR interpretation"@en;
  <http://www.w3.org/2000/01/rdf-schema#subClassOf> <https://w3id.org/fair/fip/terms/FAIR-Declaration>;
  <http://www.w3.org/2004/02/skos/core#definition> "A theoretical and practical explanation of the FAIR Principle by a recognized expert authority."@en .

<https://w3id.org/fair/fip/terms/FAIR-Qualification-Criteria> a <http://www.w3.org/2002/07/owl#Class>;
  <http://www.w3.org/2000/01/rdf-schema#isDefinedBy> <https://w3id.org/fair/fip/latest/FAIR-Qualification-Criteria>;
  <http://www.w3.org/2000/01/rdf-schema#label> "FAIR Qualifcation Criteria"@en;
  <http://www.w3.org/2000/01/rdf-schema#subClassOf> <https://w3id.org/fair/fip/terms/FAIR-Declaration>;
  <http://www.w3.org/2004/02/skos/core#definition> "A proposition on which a qualification of FAIR Supporting Resources is based."@en .

<https://w3id.org/fair/fip/terms/FAIR-Case-Study> a <http://www.w3.org/2002/07/owl#Class>;
  <http://www.w3.org/2000/01/rdf-schema#isDefinedBy> <https://w3id.org/fair/fip/latest/FAIR-Case-Study>;
  <http://www.w3.org/2000/01/rdf-schema#label> "FAIR case study"@en;
  <http://www.w3.org/2000/01/rdf-schema#subClassOf> <https://w3id.org/fair/fip/terms/FAIR-Declaration>;
  <http://www.w3.org/2004/02/skos/core#definition> "A description of a real-life situation where FAIR requirements of digital objects play a central role."@en .

<https://w3id.org/fair/fip/terms/FIP-No-Choice-Declaration> a <http://www.w3.org/2002/07/owl#Class>;
  <http://www.w3.org/2000/01/rdf-schema#isDefinedBy> <https://w3id.org/fair/fip/latest/FIP-No-Choice-Declaration>;
  <http://www.w3.org/2000/01/rdf-schema#label> "FIP No-Choice Declaration"@en;
  <http://www.w3.org/2000/01/rdf-schema#subClassOf> <https://w3id.org/fair/fip/terms/FIP-Declaration>;
  <http://www.w3.org/2004/02/skos/core#definition> "A declaration stating that no choice has been made (yet)"@en .

<https://w3id.org/fair/fip/terms/FAIR-Implementation-Community> a <http://www.w3.org/2002/07/owl#Class>;
  <http://www.w3.org/2000/01/rdf-schema#isDefinedBy> <https://w3id.org/fair/fip/latest/FAIR-Implementation-Community>;
  <http://www.w3.org/2000/01/rdf-schema#label> "FAIR Implementation Community"@en;
  <http://www.w3.org/2000/01/rdf-schema#subClassOf> <https://w3id.org/fair/fip/terms/FAIR-Supporting-Resource>;
  <http://www.w3.org/2004/02/skos/core#definition> "A FAIR Implementation Community (FIC) is a self-identified collection of people and/or organizations with the aim to implement the FAIR Principles"@en .

<https://w3id.org/fair/fip/terms/Mature-Community> a <http://www.w3.org/2002/07/owl#Class>;
  <http://www.w3.org/2000/01/rdf-schema#isDefinedBy> <https://w3id.org/fair/fip/latest/Mature-Community>;
  <http://www.w3.org/2000/01/rdf-schema#label> "Mature community"@en;
  <http://www.w3.org/2000/01/rdf-schema#subClassOf> <https://w3id.org/fair/fip/terms/FAIR-Implementation-Community>;
  <http://www.w3.org/2004/02/skos/core#definition> "A well-established community interested to implement FAIR in their data and services."@en .

<https://w3id.org/fair/fip/terms/Emerging-Community> a <http://www.w3.org/2002/07/owl#Class>;
  <http://www.w3.org/2000/01/rdf-schema#isDefinedBy> <https://w3id.org/fair/fip/latest/Emerging-Community>;
  <http://www.w3.org/2000/01/rdf-schema#label> "Emerging community"@en;
  <http://www.w3.org/2000/01/rdf-schema#subClassOf> <https://w3id.org/fair/fip/terms/FAIR-Implementation-Community>;
  <http://www.w3.org/2004/02/skos/core#definition> "An early-stage community committed to adopting and promoting FAIR principles for its data and services from the outset."@en .

<https://w3id.org/fair/fip/terms/has-data-steward> a <http://www.w3.org/1999/02/22-rdf-syntax-ns#Property>,
    <http://www.w3.org/2002/07/owl#ObjectProperty>;
  <http://www.w3.org/2000/01/rdf-schema#domain> <https://w3id.org/fair/fip/terms/FAIR-Implementation-Community>;
  <http://www.w3.org/2000/01/rdf-schema#isDefinedBy> <https://w3id.org/fair/fip/latest/has-data-steward>;
  <http://www.w3.org/2000/01/rdf-schema#label> "has data steward"@en;
  <http://www.w3.org/2000/01/rdf-schema#subPropertyOf> <http://xmlns.com/foaf/0.1/member>;
  <http://www.w3.org/2004/02/skos/core#definition> "Specifies the data steward for a FAIR implementation community"@en .

<https://w3id.org/fair/fip/terms/FAIR-Supporting-Resource> a <http://www.w3.org/2002/07/owl#Class>;
  <http://www.w3.org/2000/01/rdf-schema#isDefinedBy> <https://w3id.org/fair/fip/latest/FAIR-Supporting-Resource>;
  <http://www.w3.org/2000/01/rdf-schema#label> "FAIR Supporting Resource"@en;
  <http://www.w3.org/2004/02/skos/core#definition> "Any resource that supports FAIR Data Stewardship. FSRs are represented as FAIR Digital Objects (using the nanopublication framework) with Globally Unique, Persistent, Resolvable Identifiers (GUPRI) that resolve to machine-readable metadata about the resource."@en .

<https://w3id.org/fair/fip/terms/Available-FAIR-Supporting-Resource> a <http://www.w3.org/2002/07/owl#Class>;
  <http://www.w3.org/2000/01/rdf-schema#isDefinedBy> <https://w3id.org/fair/fip/latest/Available-FAIR-Supporting-Resource>;
  <http://www.w3.org/2000/01/rdf-schema#label> "Available FAIR Supporting Resource"@en;
  <http://www.w3.org/2000/01/rdf-schema#subClassOf> <https://w3id.org/fair/fip/terms/FAIR-Supporting-Resource>;
  <http://www.w3.org/2004/02/skos/core#definition> "A FAIR Supporting Resource that is available for use."@en .

<https://w3id.org/fair/fip/terms/FAIR-Supporting-Resource-to-be-Developed> a <http://www.w3.org/2002/07/owl#Class>;
  <http://www.w3.org/2000/01/rdf-schema#isDefinedBy> <https://w3id.org/fair/fip/latest/FAIR-Supporting-Resource-to-be-Developed>;
  <http://www.w3.org/2000/01/rdf-schema#label> "FAIR Supporting Resource to be developed"@en;
  <http://www.w3.org/2000/01/rdf-schema#subClassOf> <https://w3id.org/fair/fip/terms/FAIR-Supporting-Resource>;
  <http://www.w3.org/2004/02/skos/core#definition> "A FAIR Supporting Resource that is not yet available but still needs to be developed."@en .

<https://w3id.org/fair/fip/terms/FAIR-Enabling-Resource> a <http://www.w3.org/2002/07/owl#Class>;
  <http://www.w3.org/2000/01/rdf-schema#isDefinedBy> <https://w3id.org/fair/fip/latest/FAIR-Enabling-Resource>;
  <http://www.w3.org/2000/01/rdf-schema#label> "FAIR-Enabling Resource"@en;
  <http://www.w3.org/2000/01/rdf-schema#subClassOf> <https://w3id.org/fair/fip/terms/FAIR-Supporting-Resource>;
  <http://www.w3.org/2004/02/skos/core#definition> "A service, a specification or a data policy that is essential to the operationalization of the FAIR Principles, i.e., puts FAIR into action. A FAIR-Enabling Resource (FER) provides a function needed to achieve some aspect of FAIR behavior and is explicitly linked to one or more FAIR principles."@en .

<https://w3id.org/fair/fip/terms/FAIR-Implementation-Profile> a <http://www.w3.org/2002/07/owl#Class>;
  <http://www.w3.org/2000/01/rdf-schema#isDefinedBy> <https://w3id.org/fair/fip/latest/FAIR-Implementation-Profile>;
  <http://www.w3.org/2000/01/rdf-schema#label> "FAIR Implementation Profile"@en;
  <http://www.w3.org/2000/01/rdf-schema#subClassOf> <https://w3id.org/fair/fip/terms/FAIR-Enabling-Resource>,
    <https://w3id.org/fair/fip/terms/FAIR-Specification>;
  <http://www.w3.org/2004/02/skos/core#definition> "A FAIR Implementation Profile (FIP) is a list of declared technology choices intended to implement each of the FAIR Guiding Principles, made as a collective decision by the members of a particular community of practice."@en .

<https://w3id.org/fair/fip/terms/Reference-FAIR-Implementation-Profile> a <http://www.w3.org/2002/07/owl#Class>;
  <http://www.w3.org/2000/01/rdf-schema#isDefinedBy> <https://w3id.org/fair/fip/latest/Reference-FAIR-Implementation-Profile>;
  <http://www.w3.org/2000/01/rdf-schema#label> "Reference FAIR Implementation Profile"@en;
  <http://www.w3.org/2000/01/rdf-schema#subClassOf> <https://w3id.org/fair/fip/terms/FAIR-Implementation-Profile>;
  <http://www.w3.org/2004/02/skos/core#definition> "A list of recommended FAIR Enabling Resources intended to implement the FAIR Guiding Principles, made as a collective decision by the members of a particular community of practice."@en .

<https://w3id.org/fair/fip/terms/Available-FAIR-Enabling-Resource> a <http://www.w3.org/2002/07/owl#Class>;
  <http://www.w3.org/2000/01/rdf-schema#isDefinedBy> <https://w3id.org/fair/fip/latest/Available-FAIR-Enabling-Resource>;
  <http://www.w3.org/2000/01/rdf-schema#label> "Available FAIR-Enabling Resource"@en;
  <http://www.w3.org/2000/01/rdf-schema#subClassOf> <https://w3id.org/fair/fip/terms/Available-FAIR-Supporting-Resource>,
    <https://w3id.org/fair/fip/terms/FAIR-Enabling-Resource>;
  <http://www.w3.org/2004/02/skos/core#definition> "A FAIR-enabling resource that is available for use"@en .

<https://w3id.org/fair/fip/terms/FAIR-Enabling-Resource-to-be-Developed> a <http://www.w3.org/2002/07/owl#Class>;
  <http://www.w3.org/2000/01/rdf-schema#isDefinedBy> <https://w3id.org/fair/fip/latest/FAIR-Enabling-Resource-to-be-Developed>;
  <http://www.w3.org/2000/01/rdf-schema#label> "FAIR-Enabling Resource to be Developed"@en;
  <http://www.w3.org/2000/01/rdf-schema#subClassOf> <https://w3id.org/fair/fip/terms/FAIR-Enabling-Resource>,
    <https://w3id.org/fair/fip/terms/FAIR-Supporting-Resource-to-be-Developed>;
  <http://www.w3.org/2004/02/skos/core#definition> "A FAIR-enabling resource that is not yet available but still needs to be developed"@en .

<https://w3id.org/fair/fip/terms/FAIR-Data-Policy> a <http://www.w3.org/2002/07/owl#Class>;
  <http://www.w3.org/2000/01/rdf-schema#isDefinedBy> <https://w3id.org/fair/fip/latest/FAIR-Data-Policy>;
  <http://www.w3.org/2000/01/rdf-schema#label> "FAIR Data Policy"@en;
  <http://www.w3.org/2000/01/rdf-schema#subClassOf> <https://w3id.org/fair/fip/terms/FAIR-Supporting-Resource>;
  <http://www.w3.org/2004/02/skos/core#definition> "A policy that specifies and guides FAIR data practices for a community."@en .

<https://w3id.org/fair/fip/terms/FAIR-Data-Stewardship-Plan-Template> a <http://www.w3.org/2002/07/owl#Class>;
  <http://www.w3.org/2000/01/rdf-schema#isDefinedBy> <https://w3id.org/fair/fip/latest/FAIR-Data-Stewardship-Plan-Template>;
  <http://www.w3.org/2000/01/rdf-schema#label> "FAIR data stewardship plan template"@en;
  <http://www.w3.org/2000/01/rdf-schema#subClassOf> <https://w3id.org/fair/fip/terms/FAIR-Supporting-Resource>;
  <http://www.w3.org/2004/02/skos/core#definition> "A template guiding data stewardship including how FAIR Principles should be implemented. The template must be completed with project-specific information in any given instance to outline how data are to be handled in preparation for the project,  during the research project, and after the project is completed."@en .

<https://w3id.org/fair/fip/terms/Data-Steward-Professional-Profile> a <http://www.w3.org/2002/07/owl#Class>;
  <http://www.w3.org/2000/01/rdf-schema#isDefinedBy> <https://w3id.org/fair/fip/latest/Data-Steward-Professional-Profile>;
  <http://www.w3.org/2000/01/rdf-schema#label> "FAIR data steward professional profile"@en;
  <http://www.w3.org/2000/01/rdf-schema#subClassOf> <https://w3id.org/fair/fip/terms/FAIR-Supporting-Resource>;
  <http://www.w3.org/2004/02/skos/core#definition> "A document stating the accumulated training qualifications and FAIR outputs authored by or contributed to, by that person. The profile may be augmented with additional statements regarding professional roles and skills."@en .

<https://w3id.org/fair/fip/terms/FAIR-Data-Stewardship-Event> a <http://www.w3.org/2002/07/owl#Class>;
  <http://www.w3.org/2000/01/rdf-schema#isDefinedBy> <https://w3id.org/fair/fip/latest/FAIR-Data-Stewardship-Event>;
  <http://www.w3.org/2000/01/rdf-schema#label> "FAIR data stewardship event"@en;
  <http://www.w3.org/2000/01/rdf-schema#subClassOf> <https://w3id.org/fair/fip/terms/FAIR-Supporting-Resource>;
  <http://www.w3.org/2004/02/skos/core#definition> "A meeting specifically designed for current or aspiring data stewards to provide a rigorous understanding of the FAIR principles from theory to their concrete implementation."@en .

<https://w3id.org/fair/fip/terms/FAIR-Training-Material> a <http://www.w3.org/2002/07/owl#Class>;
  <http://www.w3.org/2000/01/rdf-schema#isDefinedBy> <https://w3id.org/fair/fip/latest/FAIR-Training-Material>;
  <http://www.w3.org/2000/01/rdf-schema#label> "FAIR training material"@en;
  <http://www.w3.org/2000/01/rdf-schema#subClassOf> <https://w3id.org/fair/fip/terms/FAIR-Supporting-Resource>;
  <http://www.w3.org/2004/02/skos/core#definition> "Any educational resource (such as the content or its published representation in text, presentation graphics, or video) that covers FAIR topics of interest."@en .

<https://w3id.org/fair/fip/terms/FAIR-Practice> a <http://www.w3.org/2002/07/owl#Class>;
  <http://www.w3.org/2000/01/rdf-schema#isDefinedBy> <https://w3id.org/fair/fip/latest/FAIR-Practice>;
  <http://www.w3.org/2000/01/rdf-schema#label> "FAIR practice"@en;
  <http://www.w3.org/2000/01/rdf-schema#subClassOf> <https://w3id.org/fair/fip/terms/FAIR-Supporting-Resource>;
  <http://www.w3.org/2004/02/skos/core#definition> "A method description detailing the use of a specific resource or a combination of resources as applied by a community to achieve FAIR processing of information."@en .

<https://w3id.org/fair/fip/terms/FAIR-Specification> a <http://www.w3.org/2002/07/owl#Class>;
  <http://www.w3.org/2000/01/rdf-schema#isDefinedBy> <https://w3id.org/fair/fip/latest/FAIR-Specification>;
  <http://www.w3.org/2000/01/rdf-schema#label> "FAIR specification"@en;
  <http://www.w3.org/2000/01/rdf-schema#subClassOf> <https://w3id.org/fair/fip/terms/FAIR-Supporting-Resource>;
  <http://www.w3.org/2004/02/skos/core#definition> "A precise description of features, requirements, constraints and recommendations for a specific implementation of a component, system or service supporting the implementation of the FAIR principles."@en .

<https://w3id.org/fair/fip/terms/Crosswalk> a <http://www.w3.org/2002/07/owl#Class>;
  <http://www.w3.org/2000/01/rdf-schema#isDefinedBy> <https://w3id.org/fair/fip/latest/Crosswalk>;
  <http://www.w3.org/2000/01/rdf-schema#label> "Crosswalk"@en;
  <http://www.w3.org/2000/01/rdf-schema#subClassOf> <https://w3id.org/fair/fip/terms/FAIR-Specification>;
  <http://www.w3.org/2004/02/skos/core#definition> "A specification consisting of a set of rules that define how (meta)data elements or attributes from one schema can be aligned and mapped to (meta)data elements or attributes in another schema that share the same constraints and thus share the same semantic role."@en .

<https://w3id.org/fair/fip/terms/FAIR-Supporting-Technology> a <http://www.w3.org/2002/07/owl#Class>;
  <http://www.w3.org/2000/01/rdf-schema#isDefinedBy> <https://w3id.org/fair/fip/latest/FAIR-Supporting-Technology>;
  <http://www.w3.org/2000/01/rdf-schema#label> "FAIR Supporting Technology"@en;
  <http://www.w3.org/2000/01/rdf-schema#subClassOf> <https://w3id.org/fair/fip/terms/FAIR-Supporting-Resource>;
  <http://www.w3.org/2004/02/skos/core#definition> "Any online accessible software system or component that supports the implementation of the FAIR Principles."@en .

<https://w3id.org/fair/fip/terms/FAIR-Supporting-Software> a <http://www.w3.org/2002/07/owl#Class>;
  <http://www.w3.org/2000/01/rdf-schema#isDefinedBy> <https://w3id.org/fair/fip/latest/FAIR-Supporting-Software>;
  <http://www.w3.org/2000/01/rdf-schema#label> "FAIR Supporting Software"@en;
  <http://www.w3.org/2000/01/rdf-schema#subClassOf> <https://w3id.org/fair/fip/terms/FAIR-Supporting-Technology>;
  <http://www.w3.org/2004/02/skos/core#definition> "Any set of machine-readable instructions that support the implementation of FAIR, that conform to a given syntax, that are interpretable by a given processor, and that instruct a computer's processor to perform specific tasks."@en .

<https://w3id.org/fair/fip/terms/FAIR-Representation-Service> a <http://www.w3.org/2002/07/owl#Class>;
  <http://www.w3.org/2000/01/rdf-schema#isDefinedBy> <https://w3id.org/fair/fip/latest/FAIR-Representation-Service>;
  <http://www.w3.org/2000/01/rdf-schema#label> "FAIR Representation Service"@en;
  <http://www.w3.org/2000/01/rdf-schema#subClassOf> <https://w3id.org/fair/fip/terms/FAIR-Supporting-Technology>;
  <http://www.w3.org/2004/02/skos/core#definition> "A transformation service that converts non-FAIR data into a FAIR representation using machine-readable knowledge representation languages."@en .

<https://w3id.org/fair/fip/terms/Web-API> a <http://www.w3.org/2002/07/owl#Class>;
  <http://www.w3.org/2000/01/rdf-schema#isDefinedBy> <https://w3id.org/fair/fip/latest/Web-API>;
  <http://www.w3.org/2000/01/rdf-schema#label> "Web-API"@en;
  <http://www.w3.org/2000/01/rdf-schema#subClassOf> <https://w3id.org/fair/fip/terms/FAIR-Supporting-Technology>;
  <http://www.w3.org/2004/02/skos/core#definition> "An Application Programming Interface (API) for the World Wide Web that allows different software applications to communicate with each other."@en .

<https://w3id.org/fair/fip/terms/Editor> a <http://www.w3.org/2002/07/owl#Class>;
  <http://www.w3.org/2000/01/rdf-schema#isDefinedBy> <https://w3id.org/fair/fip/latest/Editor>;
  <http://www.w3.org/2000/01/rdf-schema#label> "Editor"@en;
  <http://www.w3.org/2000/01/rdf-schema#subClassOf> <https://w3id.org/fair/fip/terms/FAIR-Supporting-Technology>;
  <http://www.w3.org/2004/02/skos/core#definition> "A service that provides a user-friendly interface for easy editing of metadata, vocabularies or crosswalks."@en .

<https://w3id.org/fair/fip/terms/Validation-Service> a <http://www.w3.org/2002/07/owl#Class>;
  <http://www.w3.org/2000/01/rdf-schema#isDefinedBy> <https://w3id.org/fair/fip/latest/Validation-Service>;
  <http://www.w3.org/2000/01/rdf-schema#label> "Validation service"@en;
  <http://www.w3.org/2000/01/rdf-schema#subClassOf> <https://w3id.org/fair/fip/terms/FAIR-Supporting-Technology>;
  <http://www.w3.org/2004/02/skos/core#definition> "A system that automatically verifies the accuracy, completeness, or compliance of data, code or processes against predefined criteria or standards."@en .

<https://w3id.org/fair/fip/terms/Provenance-Tracking-Service> a <http://www.w3.org/2002/07/owl#Class>;
  <http://www.w3.org/2000/01/rdf-schema#isDefinedBy> <https://w3id.org/fair/fip/latest/Provenance-Tracking-Service>;
  <http://www.w3.org/2000/01/rdf-schema#label> "Provenance tracking service"@en;
  <http://www.w3.org/2000/01/rdf-schema#subClassOf> <https://w3id.org/fair/fip/terms/FAIR-Supporting-Technology>;
  <http://www.w3.org/2004/02/skos/core#definition> "A system that systematically captures, stores and manages detailed information about the origin, history, and lifecycle of digital objects creating metadata based on a provenance model. "@en .

<https://w3id.org/fair/fip/terms/Semantic-Interoperability-Profile> a <http://www.w3.org/2002/07/owl#Class>;
  <http://www.w3.org/2000/01/rdf-schema#isDefinedBy> <https://w3id.org/fair/fip/latest/Semantic-Interoperability-Profile>;
  <http://www.w3.org/2000/01/rdf-schema#label> "Semantic Interoperability Profile"@en;
  <http://www.w3.org/2000/01/rdf-schema#subClassOf> <https://w3id.org/fair/fip/terms/FAIR-Supporting-Resource>;
  <http://www.w3.org/2004/02/skos/core#definition> "A Semantic Interoperability Profil (SIP) is a list of FAIR Supporting Resources chosen by a community to support semantic interoperability of (meta)data."@en .

<https://w3id.org/fair/fip/terms/Digital-Object-Type> a <http://www.w3.org/2002/07/owl#Class>;
  <http://www.w3.org/2000/01/rdf-schema#isDefinedBy> <https://w3id.org/fair/fip/latest/Digital-Object-Type>;
  <http://www.w3.org/2000/01/rdf-schema#label> "Digital Object Type"@en;
  <http://www.w3.org/2004/02/skos/core#definition> "A digital object type is a classification of digital objects with respect to their informational functions to specify the nature of the digital object and the operations that can be performed on it."@en .

<https://w3id.org/fair/fip/terms/Identifier-service> a <http://www.w3.org/2002/07/owl#Class>;
  <http://www.w3.org/2000/01/rdf-schema#isDefinedBy> <https://w3id.org/fair/fip/latest/Identifier-service>;
  <http://www.w3.org/2000/01/rdf-schema#label> "Identifier service"@en;
  <http://www.w3.org/2000/01/rdf-schema#subClassOf> <https://w3id.org/fair/fip/terms/FAIR-Enabling-Resource>,
    <https://w3id.org/fair/fip/terms/FAIR-Supporting-Technology>;
  <http://www.w3.org/2004/02/skos/core#definition> "A service that provides for any digital object (1) algorithms guaranteeing global uniqueness, (2) policy document that guarantees persistent and (3) resolution of the identifier to machine-actionable metadata describing the object and its location."@en .

<https://w3id.org/fair/fip/terms/Metadata-schema> a <http://www.w3.org/2002/07/owl#Class>;
  <http://www.w3.org/2000/01/rdf-schema#isDefinedBy> <https://w3id.org/fair/fip/latest/Metadata-schema>;
  <http://www.w3.org/2000/01/rdf-schema#label> "Metadata schema"@en;
  <http://www.w3.org/2000/01/rdf-schema#subClassOf> <https://w3id.org/fair/fip/terms/FAIR-Enabling-Resource>,
    <https://w3id.org/fair/fip/terms/FAIR-Specification>;
  <http://www.w3.org/2004/02/skos/core#definition> "A specification that specifies the structured representation of metadata describing attributes of data or other digital objects in terms of semantics, syntax and optionality."@en .

<https://w3id.org/fair/fip/terms/Metadata-data-linking-schema> a <http://www.w3.org/2002/07/owl#Class>;
  <http://www.w3.org/2000/01/rdf-schema#isDefinedBy> <https://w3id.org/fair/fip/latest/Metadata-data-linking-schema>;
  <http://www.w3.org/2000/01/rdf-schema#label> "Metadata-data linking schema"@en;
  <http://www.w3.org/2000/01/rdf-schema#subClassOf> <https://w3id.org/fair/fip/terms/FAIR-Enabling-Resource>,
    <https://w3id.org/fair/fip/terms/FAIR-Specification>;
  <http://www.w3.org/2004/02/skos/core#definition> "A specification that provides a unique, persistent, (ideally) bi-directional, machine-actionable link between metadata and the data they describe."@en .

<https://w3id.org/fair/fip/terms/Registry> a <http://www.w3.org/2002/07/owl#Class>;
  <http://www.w3.org/2000/01/rdf-schema#isDefinedBy> <https://w3id.org/fair/fip/latest/Registry>;
  <http://www.w3.org/2000/01/rdf-schema#label> "Registry"@en;
  <http://www.w3.org/2000/01/rdf-schema#subClassOf> <https://w3id.org/fair/fip/terms/FAIR-Enabling-Resource>,
    <https://w3id.org/fair/fip/terms/FAIR-Supporting-Technology>;
  <http://www.w3.org/2004/02/skos/core#definition> "A service that indexes metadata and data and provides search over that index."@en .

<https://w3id.org/fair/fip/terms/Generalist-Registry> a <http://www.w3.org/2002/07/owl#Class>;
  <http://www.w3.org/2000/01/rdf-schema#isDefinedBy> <https://w3id.org/fair/fip/latest/Generalist-Registry>;
  <http://www.w3.org/2000/01/rdf-schema#label> "Generalist registry"@en;
  <http://www.w3.org/2000/01/rdf-schema#subClassOf> <https://w3id.org/fair/fip/terms/Registry>;
  <http://www.w3.org/2004/02/skos/core#definition> "A registry designed to collect, provide access to, and enable searching of data without any restrictions on the domain."@en .

<https://w3id.org/fair/fip/terms/Domain-Specific-Registry> a <http://www.w3.org/2002/07/owl#Class>;
  <http://www.w3.org/2000/01/rdf-schema#isDefinedBy> <https://w3id.org/fair/fip/latest/Domain-Specific-Registry>;
  <http://www.w3.org/2000/01/rdf-schema#label> "Domain-specific registry"@en;
  <http://www.w3.org/2000/01/rdf-schema#subClassOf> <https://w3id.org/fair/fip/terms/Registry>;
  <http://www.w3.org/2004/02/skos/core#definition> "A registry designed to collect, provide access to, and enable searching of data within a particular domain or subject area"@en .

<https://w3id.org/fair/fip/terms/Communication-protocol> a <http://www.w3.org/2002/07/owl#Class>;
  <http://www.w3.org/2000/01/rdf-schema#isDefinedBy> <https://w3id.org/fair/fip/latest/Communication-protocol>;
  <http://www.w3.org/2000/01/rdf-schema#label> "Communication protocol"@en;
  <http://www.w3.org/2000/01/rdf-schema#subClassOf> <https://w3id.org/fair/fip/terms/FAIR-Enabling-Resource>,
    <https://w3id.org/fair/fip/terms/FAIR-Specification>;
  <http://www.w3.org/2004/02/skos/core#definition> "A specification of how messages are structured and exchanged."@en .

<https://w3id.org/fair/fip/terms/Authentication-and-authorization-service> a <http://www.w3.org/2002/07/owl#Class>;
  <http://www.w3.org/2000/01/rdf-schema#isDefinedBy> <https://w3id.org/fair/fip/latest/Authentication-and-authorization-service>;
  <http://www.w3.org/2000/01/rdf-schema#label> "Authentication and authorization service"@en;
  <http://www.w3.org/2000/01/rdf-schema#subClassOf> <https://w3id.org/fair/fip/terms/FAIR-Enabling-Resource>,
    <https://w3id.org/fair/fip/terms/FAIR-Supporting-Technology>;
  <http://www.w3.org/2004/02/skos/core#definition> "A service that mediates access to digital objects according to specifed conditions."@en .

<https://w3id.org/fair/fip/terms/Metadata-preservation-policy> a <http://www.w3.org/2002/07/owl#Class>;
  <http://www.w3.org/2000/01/rdf-schema#isDefinedBy> <https://w3id.org/fair/fip/latest/Metadata-preservation-policy>;
  <http://www.w3.org/2000/01/rdf-schema#label> "Metadata preservation policy"@en;
  <http://www.w3.org/2000/01/rdf-schema#subClassOf> <https://w3id.org/fair/fip/terms/FAIR-Data-Policy>,
    <https://w3id.org/fair/fip/terms/FAIR-Enabling-Resource>;
  <http://www.w3.org/2004/02/skos/core#definition> "A data policy that describes the conditions under which metadata should be provided in the future."@en .

<https://w3id.org/fair/fip/terms/Knowledge-representation-language> a <http://www.w3.org/2002/07/owl#Class>;
  <http://www.w3.org/2000/01/rdf-schema#isDefinedBy> <https://w3id.org/fair/fip/latest/Knowledge-representation-language>;
  <http://www.w3.org/2000/01/rdf-schema#label> "Knowledge representation language"@en;
  <http://www.w3.org/2000/01/rdf-schema#subClassOf> <https://w3id.org/fair/fip/terms/FAIR-Enabling-Resource>,
    <https://w3id.org/fair/fip/terms/FAIR-Specification>;
  <http://www.w3.org/2004/02/skos/core#definition> "A language specification that enables knowledge to be processed by machines."@en .

<https://w3id.org/fair/fip/terms/Structured-vocabulary> a <http://www.w3.org/2002/07/owl#Class>;
  <http://www.w3.org/2000/01/rdf-schema#isDefinedBy> <https://w3id.org/fair/fip/latest/Structured-vocabulary>;
  <http://www.w3.org/2000/01/rdf-schema#label> "Structured vocabulary"@en;
  <http://www.w3.org/2000/01/rdf-schema#subClassOf> <https://w3id.org/fair/fip/terms/FAIR-Enabling-Resource>,
    <https://w3id.org/fair/fip/terms/FAIR-Specification>;
  <http://www.w3.org/2004/02/skos/core#definition> "A specification for a controlled list of uniquely identified and unambigous concepts with their definitions represented using web standards."@en .

<https://w3id.org/fair/fip/terms/Semantic-model> a <http://www.w3.org/2002/07/owl#Class>;
  <http://www.w3.org/2000/01/rdf-schema#isDefinedBy> <https://w3id.org/fair/fip/latest/Semantic-model>;
  <http://www.w3.org/2000/01/rdf-schema#label> "Semantic model"@en;
  <http://www.w3.org/2000/01/rdf-schema#subClassOf> <https://w3id.org/fair/fip/terms/FAIR-Enabling-Resource>,
    <https://w3id.org/fair/fip/terms/FAIR-Specification>;
  <http://www.w3.org/2004/02/skos/core#definition> "A specification that defines qualified relations between entities describing data or other digital objects according to the Linked Data principles. This can include semantic data models and ontologies."@en .

<https://w3id.org/fair/fip/terms/Data-usage-license> a <http://www.w3.org/2002/07/owl#Class>;
  <http://www.w3.org/2000/01/rdf-schema#isDefinedBy> <https://w3id.org/fair/fip/latest/Data-usage-license>;
  <http://www.w3.org/2000/01/rdf-schema#label> "Data usage license"@en;
  <http://www.w3.org/2000/01/rdf-schema#subClassOf> <https://w3id.org/fair/fip/terms/FAIR-Data-Policy>,
    <https://w3id.org/fair/fip/terms/FAIR-Enabling-Resource>;
  <http://www.w3.org/2004/02/skos/core#definition> "A data policy that specifies legal restrictions on the reuse of the data."@en .

<https://w3id.org/fair/fip/terms/Persistency-Policy> a <http://www.w3.org/2002/07/owl#Class>;
  <http://www.w3.org/2000/01/rdf-schema#isDefinedBy> <https://w3id.org/fair/fip/latest/Persistency-Policy>;
  <http://www.w3.org/2000/01/rdf-schema#label> "Persistency Policy"@en;
  <http://www.w3.org/2000/01/rdf-schema#subClassOf> <https://w3id.org/fair/fip/terms/FAIR-Data-Policy>,
    <https://w3id.org/fair/fip/terms/FAIR-Enabling-Resource>;
  <http://www.w3.org/2004/02/skos/core#definition> "A policy with respect to persistency of resources."@en .

<https://w3id.org/fair/fip/terms/Provenance-model> a <http://www.w3.org/2002/07/owl#Class>;
  <http://www.w3.org/2000/01/rdf-schema#isDefinedBy> <https://w3id.org/fair/fip/latest/Provenance-model>;
  <http://www.w3.org/2000/01/rdf-schema#label> "Provenance model"@en;
  <http://www.w3.org/2000/01/rdf-schema#subClassOf> <https://w3id.org/fair/fip/terms/FAIR-Enabling-Resource>,
    <https://w3id.org/fair/fip/terms/FAIR-Specification>;
  <http://www.w3.org/2004/02/skos/core#definition> "A specification that specifies metadata describing the origin and lineage of data or other digital objects."@en .

<https://w3id.org/fair/fip/terms/refers-to-principle> a <http://www.w3.org/1999/02/22-rdf-syntax-ns#Property>,
    <http://www.w3.org/2002/07/owl#ObjectProperty>;
  <http://www.w3.org/2000/01/rdf-schema#isDefinedBy> <https://w3id.org/fair/fip/latest/refers-to-principle>;
  <http://www.w3.org/2000/01/rdf-schema#label> "refers to principle"@en;
  <http://www.w3.org/2000/01/rdf-schema#range> <https://w3id.org/fair/principles/terms/FAIR-Principle-or-SubPrinciple>;
  <http://www.w3.org/2004/02/skos/core#definition> "Connects an entity (for example a FIP declaration) to a FAIR (sub)principle it refers to"@en .

<https://w3id.org/fair/fip/terms/refers-to-question> a <http://www.w3.org/1999/02/22-rdf-syntax-ns#Property>,
    <http://www.w3.org/2002/07/owl#ObjectProperty>;
  <http://www.w3.org/2000/01/rdf-schema#domain> <https://w3id.org/fair/fip/terms/FIP-Declaration>;
  <http://www.w3.org/2000/01/rdf-schema#isDefinedBy> <https://w3id.org/fair/fip/latest/refers-to-question>;
  <http://www.w3.org/2000/01/rdf-schema#label> "refers to question"@en;
  <http://www.w3.org/2000/01/rdf-schema#range> <https://w3id.org/fair/fip/terms/FIP-Question>;
  <http://www.w3.org/2004/02/skos/core#definition> "Connects a FIP declaration to the FIP question it is addressing"@en .

<https://w3id.org/fair/fip/terms/declared-by> a <http://www.w3.org/1999/02/22-rdf-syntax-ns#Property>,
    <http://www.w3.org/2002/07/owl#ObjectProperty>;
  <http://www.w3.org/2000/01/rdf-schema#domain> <https://w3id.org/fair/fip/terms/FAIR-Declaration>;
  <http://www.w3.org/2000/01/rdf-schema#isDefinedBy> <https://w3id.org/fair/fip/latest/declared-by>;
  <http://www.w3.org/2000/01/rdf-schema#label> "declared by"@en;
  <http://www.w3.org/2000/01/rdf-schema#range> <https://w3id.org/fair/fip/terms/FAIR-Implementation-Community>;
  <http://www.w3.org/2004/02/skos/core#definition> "Connects a FIP declaration to the community that made the declaration"@en .

<https://w3id.org/fair/fip/terms/declares-current-use-of> a <http://www.w3.org/1999/02/22-rdf-syntax-ns#Property>,
    <http://www.w3.org/2002/07/owl#ObjectProperty>;
  <http://www.w3.org/2000/01/rdf-schema#domain> <https://w3id.org/fair/fip/terms/FAIR-Declaration>;
  <http://www.w3.org/2000/01/rdf-schema#isDefinedBy> <https://w3id.org/fair/fip/latest/declares-current-use-of>;
  <http://www.w3.org/2000/01/rdf-schema#label> "declares current use of"@en;
  <http://www.w3.org/2000/01/rdf-schema#range> <https://w3id.org/fair/fip/terms/Available-FAIR-Supporting-Resource>;
  <http://www.w3.org/2004/02/skos/core#definition> "Connects a FIP declaration to the resource that the community thereby declares to currently use"@en .

<https://w3id.org/fair/fip/terms/declares-planned-use-of> a <http://www.w3.org/1999/02/22-rdf-syntax-ns#Property>,
    <http://www.w3.org/2002/07/owl#ObjectProperty>;
  <http://www.w3.org/2000/01/rdf-schema#domain> <https://w3id.org/fair/fip/terms/FAIR-Declaration>;
  <http://www.w3.org/2000/01/rdf-schema#isDefinedBy> <https://w3id.org/fair/fip/latest/declares-planned-use-of>;
  <http://www.w3.org/2000/01/rdf-schema#label> "declares planned use of"@en;
  <http://www.w3.org/2000/01/rdf-schema#range> <https://w3id.org/fair/fip/terms/FAIR-Supporting-Resource>;
  <http://www.w3.org/2004/02/skos/core#definition> "Connects a FIP declaration to the resource that the community thereby declares to plan to use in the future"@en .

<https://w3id.org/fair/fip/terms/declares-planned-replacement-of> a <http://www.w3.org/1999/02/22-rdf-syntax-ns#Property>,
    <http://www.w3.org/2002/07/owl#ObjectProperty>;
  <http://www.w3.org/2000/01/rdf-schema#domain> <https://w3id.org/fair/fip/terms/FAIR-Declaration>;
  <http://www.w3.org/2000/01/rdf-schema#isDefinedBy> <https://w3id.org/fair/fip/latest/declares-planned-replacement-of>;
  <http://www.w3.org/2000/01/rdf-schema#label> "declares planned replacement of"@en;
  <http://www.w3.org/2000/01/rdf-schema#range> <https://w3id.org/fair/fip/terms/Available-FAIR-Supporting-Resource>;
  <http://www.w3.org/2004/02/skos/core#definition> "Connects a FIP declaration to the resource that the community thereby declares to plan to replace in the future. The same declaration should also state a resource that the community declares to plan to use instead (with fip:declares-planned-use-of)."@en .

<https://w3id.org/fair/fip/terms/declares-planned-development-of> a <http://www.w3.org/1999/02/22-rdf-syntax-ns#Property>,
    <http://www.w3.org/2002/07/owl#ObjectProperty>;
  <http://www.w3.org/2000/01/rdf-schema#domain> <https://w3id.org/fair/fip/terms/FAIR-Declaration>;
  <http://www.w3.org/2000/01/rdf-schema#isDefinedBy> <https://w3id.org/fair/fip/latest/declares-planned-development-of>;
  <http://www.w3.org/2000/01/rdf-schema#label> "declares planned development of"@en;
  <http://www.w3.org/2000/01/rdf-schema#range> <https://w3id.org/fair/fip/terms/FAIR-Supporting-Resource-to-be-Developed>;
  <http://www.w3.org/2004/02/skos/core#definition> "Connects a FIP declaration to the resource that the community thereby declares to plan to develop"@en .

<https://w3id.org/fair/fip/terms/declared-for-digital-object-type> a <http://www.w3.org/1999/02/22-rdf-syntax-ns#Property>,
    <http://www.w3.org/2002/07/owl#ObjectProperty>;
  <http://www.w3.org/2000/01/rdf-schema#domain> <https://w3id.org/fair/fip/terms/FAIR-Declaration>;
  <http://www.w3.org/2000/01/rdf-schema#isDefinedBy> <https://w3id.org/fair/fip/latest/declared-for-digital-object-type>;
  <http://www.w3.org/2000/01/rdf-schema#label> "declared for digital object type"@en;
  <http://www.w3.org/2000/01/rdf-schema#range> <https://w3id.org/fair/fip/terms/Digital-Object-Type>;
  <http://www.w3.org/2004/02/skos/core#definition> "Connects a FIP declaration to the digital object type it applies to"@en .

<https://w3id.org/fair/fip/terms/declared-for-case-study> a <http://www.w3.org/1999/02/22-rdf-syntax-ns#Property>,
    <http://www.w3.org/2002/07/owl#ObjectProperty>;
  <http://www.w3.org/2000/01/rdf-schema#domain> <https://w3id.org/fair/fip/terms/FAIR-Declaration>;
  <http://www.w3.org/2000/01/rdf-schema#isDefinedBy> <https://w3id.org/fair/fip/latest/declared-for-case-study>;
  <http://www.w3.org/2000/01/rdf-schema#label> "declared for case study"@en;
  <http://www.w3.org/2000/01/rdf-schema#range> <https://w3id.org/fair/fip/terms/FAIR-Case-Study>;
  <http://www.w3.org/2004/02/skos/core#definition> "Connects a FIP declaration to the case study it refers to."@en .

<https://w3id.org/fair/fip/terms/has-declaration-index> a <http://www.w3.org/1999/02/22-rdf-syntax-ns#Property>,
    <http://www.w3.org/2002/07/owl#ObjectProperty>;
  <http://www.w3.org/2000/01/rdf-schema#domain> <https://w3id.org/fair/fip/terms/FAIR-Supporting-Resource>;
  <http://www.w3.org/2000/01/rdf-schema#isDefinedBy> <https://w3id.org/fair/fip/latest/has-declaration-index>;
  <http://www.w3.org/2000/01/rdf-schema#label> "has declaration index"@en;
  <http://www.w3.org/2000/01/rdf-schema#range> <http://purl.org/nanopub/x/NanopubIndex>;
  <http://www.w3.org/2004/02/skos/core#definition> "Connects a FAIR Implementation Profile or a Semantic Interoperability Profile to the index of their declarations."@en .

<https://w3id.org/fair/fip/terms/has-research-domain> a <http://www.w3.org/1999/02/22-rdf-syntax-ns#Property>,
    <http://www.w3.org/2002/07/owl#ObjectProperty>;
  <http://www.w3.org/2000/01/rdf-schema#domain> <https://w3id.org/fair/fip/terms/FAIR-Implementation-Community>;
  <http://www.w3.org/2000/01/rdf-schema#isDefinedBy> <https://w3id.org/fair/fip/latest/has-research-domain>;
  <http://www.w3.org/2000/01/rdf-schema#label> "has research domain"@en;
  <http://www.w3.org/2004/02/skos/core#definition> "Connects a FAIR Implementation Community with research domains"@en .

<https://w3id.org/fair/fip/terms/enables> a <http://www.w3.org/1999/02/22-rdf-syntax-ns#Property>,
    <http://www.w3.org/2002/07/owl#ObjectProperty>;
  <http://www.w3.org/2000/01/rdf-schema#domain> <http://www.w3.org/2002/07/owl#Class>;
  <http://www.w3.org/2000/01/rdf-schema#isDefinedBy> <https://w3id.org/fair/fip/latest/enables>;
  <http://www.w3.org/2000/01/rdf-schema#label> "enables"@en;
  <http://www.w3.org/2000/01/rdf-schema#range> <https://w3id.org/fair/principles/terms/FAIR-Principle-or-SubPrinciple>;
  <http://www.w3.org/2004/02/skos/core#definition> "Connects a FAIR Enabling Resource class with the FAIR principles it enables"@en .

<https://w3id.org/fair/fip/terms/considerations> a <http://www.w3.org/1999/02/22-rdf-syntax-ns#Property>,
    <http://www.w3.org/2002/07/owl#DatatypeProperty>;
  <http://www.w3.org/2000/01/rdf-schema#domain> <https://w3id.org/fair/fip/terms/FAIR-Declaration>;
  <http://www.w3.org/2000/01/rdf-schema#isDefinedBy> <https://w3id.org/fair/fip/latest/considerations>;
  <http://www.w3.org/2000/01/rdf-schema#label> "considerations"@en;
  <http://www.w3.org/2004/02/skos/core#definition> "Considerations that led to a given FIP declaration"@en .

<https://w3id.org/fair/fip/terms/availability-in-years> a <http://www.w3.org/1999/02/22-rdf-syntax-ns#Property>,
    <http://www.w3.org/2002/07/owl#DatatypeProperty>;
  <http://www.w3.org/2000/01/rdf-schema#domain> <https://w3id.org/fair/fip/terms/fip:FAIR-Data-Policy>;
  <http://www.w3.org/2000/01/rdf-schema#isDefinedBy> <https://w3id.org/fair/fip/latest/availability-in-years>;
  <http://www.w3.org/2000/01/rdf-schema#label> "availability in years"@en;
  <http://www.w3.org/2004/02/skos/core#definition> "Specifies how many years a resource is preserved according to a preservation policy"@en .

<https://w3id.org/fair/fip/terms/metadata-availability-in-years> a <http://www.w3.org/1999/02/22-rdf-syntax-ns#Property>,
    <http://www.w3.org/2002/07/owl#DatatypeProperty>;
  <http://www.w3.org/2000/01/rdf-schema#domain> <https://w3id.org/fair/fip/terms/Metadata-preservation-policy>;
  <http://www.w3.org/2000/01/rdf-schema#isDefinedBy> <https://w3id.org/fair/fip/latest/metadata-availability-in-years>;
  <http://www.w3.org/2000/01/rdf-schema#label> "metadata availability in years"@en;
  <http://www.w3.org/2000/01/rdf-schema#subPropertyOf> <https://w3id.org/fair/fip/terms/availability-in-years>;
  <http://www.w3.org/2004/02/skos/core#definition> "Specifies how many years metadata are preserved according to the metadata preservation policy"@en .

<https://w3id.org/fair/fip/terms/FIP-Question-F1-MD> a <http://www.w3.org/2002/07/owl#NamedIndividual>,
    <https://w3id.org/fair/fip/terms/FIP-Question>;
  <http://www.w3.org/2000/01/rdf-schema#isDefinedBy> <https://w3id.org/fair/fip/latest/FIP-Question-F1-MD>;
  <http://www.w3.org/2000/01/rdf-schema#label> "FIP Question F1-MD"@en;
  <http://www.w3.org/2004/02/skos/core#definition> "What globally unique, persistent, resolvable identifiers do you use for metadata records?"@en;
  <https://w3id.org/fair/fip/terms/refers-to-principle> <https://w3id.org/fair/principles/terms/F1> .

<https://w3id.org/fair/fip/terms/FIP-Question-F1-D> a <http://www.w3.org/2002/07/owl#NamedIndividual>,
    <https://w3id.org/fair/fip/terms/FIP-Question>;
  <http://www.w3.org/2000/01/rdf-schema#isDefinedBy> <https://w3id.org/fair/fip/latest/FIP-Question-F1-D>;
  <http://www.w3.org/2000/01/rdf-schema#label> "FIP Question F1-D"@en;
  <http://www.w3.org/2004/02/skos/core#definition> "What globally unique, persistent, resolvable identifiers do you use for datasets?"@en;
  <https://w3id.org/fair/fip/terms/refers-to-principle> <https://w3id.org/fair/principles/terms/F1> .

<https://w3id.org/fair/fip/terms/FIP-Question-F2> a <http://www.w3.org/2002/07/owl#NamedIndividual>,
    <https://w3id.org/fair/fip/terms/FIP-Question>;
  <http://www.w3.org/2000/01/rdf-schema#isDefinedBy> <https://w3id.org/fair/fip/latest/FIP-Question-F2>;
  <http://www.w3.org/2000/01/rdf-schema#label> "FIP Question F2"@en;
  <http://www.w3.org/2004/02/skos/core#definition> "Which metadata schemas do you use for findability?"@en;
  <https://w3id.org/fair/fip/terms/refers-to-principle> <https://w3id.org/fair/principles/terms/F2> .

<https://w3id.org/fair/fip/terms/FIP-Question-F3> a <http://www.w3.org/2002/07/owl#NamedIndividual>,
    <https://w3id.org/fair/fip/terms/FIP-Question>;
  <http://www.w3.org/2000/01/rdf-schema#isDefinedBy> <https://w3id.org/fair/fip/latest/FIP-Question-F3>;
  <http://www.w3.org/2000/01/rdf-schema#label> "FIP Question F3"@en;
  <http://www.w3.org/2004/02/skos/core#definition> "What is the technology that links the persistent identifiers of your data to the metadata description?"@en;
  <https://w3id.org/fair/fip/terms/refers-to-principle> <https://w3id.org/fair/principles/terms/F3> .

<https://w3id.org/fair/fip/terms/FIP-Question-F4-MD> a <http://www.w3.org/2002/07/owl#NamedIndividual>,
    <https://w3id.org/fair/fip/terms/FIP-Question>;
  <http://www.w3.org/2000/01/rdf-schema#isDefinedBy> <https://w3id.org/fair/fip/latest/FIP-Question-F4-MD>;
  <http://www.w3.org/2000/01/rdf-schema#label> "FIP Question F4-MD"@en;
  <http://www.w3.org/2004/02/skos/core#definition> "In which search engines are your metadata records indexed?"@en;
  <https://w3id.org/fair/fip/terms/refers-to-principle> <https://w3id.org/fair/principles/terms/F4> .

<https://w3id.org/fair/fip/terms/FIP-Question-F4-D> a <http://www.w3.org/2002/07/owl#NamedIndividual>,
    <https://w3id.org/fair/fip/terms/FIP-Question>;
  <http://www.w3.org/2000/01/rdf-schema#isDefinedBy> <https://w3id.org/fair/fip/latest/FIP-Question-F4-D>;
  <http://www.w3.org/2000/01/rdf-schema#label> "FIP Question F4-D"@en;
  <http://www.w3.org/2004/02/skos/core#definition> "In which search engines are your datasets indexed?"@en;
  <https://w3id.org/fair/fip/terms/refers-to-principle> <https://w3id.org/fair/principles/terms/F4> .

<https://w3id.org/fair/fip/terms/FIP-Question-A1.1-MD> a <http://www.w3.org/2002/07/owl#NamedIndividual>,
    <https://w3id.org/fair/fip/terms/FIP-Question>;
  <http://www.w3.org/2000/01/rdf-schema#isDefinedBy> <https://w3id.org/fair/fip/latest/FIP-Question-A1.1-MD>;
  <http://www.w3.org/2000/01/rdf-schema#label> "FIP Question A1.1-MD"@en;
  <http://www.w3.org/2004/02/skos/core#definition> "Which standardized communication protocol do you use for metadata records?"@en;
  <https://w3id.org/fair/fip/terms/refers-to-principle> <https://w3id.org/fair/principles/terms/A1.1> .

<https://w3id.org/fair/fip/terms/FIP-Question-A1.1-D> a <http://www.w3.org/2002/07/owl#NamedIndividual>,
    <https://w3id.org/fair/fip/terms/FIP-Question>;
  <http://www.w3.org/2000/01/rdf-schema#isDefinedBy> <https://w3id.org/fair/fip/latest/FIP-Question-A1.1-D>;
  <http://www.w3.org/2000/01/rdf-schema#label> "FIP Question A1.1-D"@en;
  <http://www.w3.org/2004/02/skos/core#definition> "Which standardized communication protocol do you use for datasets?"@en;
  <https://w3id.org/fair/fip/terms/refers-to-principle> <https://w3id.org/fair/principles/terms/A1.1> .

<https://w3id.org/fair/fip/terms/FIP-Question-A1.2-MD> a <http://www.w3.org/2002/07/owl#NamedIndividual>,
    <https://w3id.org/fair/fip/terms/FIP-Question>;
  <http://www.w3.org/2000/01/rdf-schema#isDefinedBy> <https://w3id.org/fair/fip/latest/FIP-Question-A1.2-MD>;
  <http://www.w3.org/2000/01/rdf-schema#label> "FIP Question A1.2-MD"@en;
  <http://www.w3.org/2004/02/skos/core#definition> "Which authentication & authorisation technique do you use for metadata records?"@en;
  <https://w3id.org/fair/fip/terms/refers-to-principle> <https://w3id.org/fair/principles/terms/A1.2> .

<https://w3id.org/fair/fip/terms/FIP-Question-A1.2-D> a <http://www.w3.org/2002/07/owl#NamedIndividual>,
    <https://w3id.org/fair/fip/terms/FIP-Question>;
  <http://www.w3.org/2000/01/rdf-schema#isDefinedBy> <https://w3id.org/fair/fip/latest/FIP-Question-A1.2-D>;
  <http://www.w3.org/2000/01/rdf-schema#label> "FIP Question A1.2-D"@en;
  <http://www.w3.org/2004/02/skos/core#definition> "Which authentication & authorisation technique do you use for datasets?"@en;
  <https://w3id.org/fair/fip/terms/refers-to-principle> <https://w3id.org/fair/principles/terms/A1.2> .

<https://w3id.org/fair/fip/terms/FIP-Question-A2> a <http://www.w3.org/2002/07/owl#NamedIndividual>,
    <https://w3id.org/fair/fip/terms/FIP-Question>;
  <http://www.w3.org/2000/01/rdf-schema#isDefinedBy> <https://w3id.org/fair/fip/latest/FIP-Question-A2>;
  <http://www.w3.org/2000/01/rdf-schema#label> "FIP Question A2"@en;
  <http://www.w3.org/2004/02/skos/core#definition> "Which metadata longevity plan do you use?"@en;
  <https://w3id.org/fair/fip/terms/refers-to-principle> <https://w3id.org/fair/principles/terms/A2> .

<https://w3id.org/fair/fip/terms/FIP-Question-I1-MD> a <http://www.w3.org/2002/07/owl#NamedIndividual>,
    <https://w3id.org/fair/fip/terms/FIP-Question>;
  <http://www.w3.org/2000/01/rdf-schema#isDefinedBy> <https://w3id.org/fair/fip/latest/FIP-Question-I1-MD>;
  <http://www.w3.org/2000/01/rdf-schema#label> "FIP Question I1-MD"@en;
  <http://www.w3.org/2004/02/skos/core#definition> "Which knowledge representation languages (allowing machine interoperation) do you use for metadata records?"@en;
  <https://w3id.org/fair/fip/terms/refers-to-principle> <https://w3id.org/fair/principles/terms/I1> .

<https://w3id.org/fair/fip/terms/FIP-Question-I1-D> a <http://www.w3.org/2002/07/owl#NamedIndividual>,
    <https://w3id.org/fair/fip/terms/FIP-Question>;
  <http://www.w3.org/2000/01/rdf-schema#isDefinedBy> <https://w3id.org/fair/fip/latest/FIP-Question-I1-D>;
  <http://www.w3.org/2000/01/rdf-schema#label> "FIP Question I1-D"@en;
  <http://www.w3.org/2004/02/skos/core#definition> "Which knowledge representation languages (allowing machine interoperation) do you use for datasets?"@en;
  <https://w3id.org/fair/fip/terms/refers-to-principle> <https://w3id.org/fair/principles/terms/I1> .

<https://w3id.org/fair/fip/terms/FIP-Question-I2-MD> a <http://www.w3.org/2002/07/owl#NamedIndividual>,
    <https://w3id.org/fair/fip/terms/FIP-Question>;
  <http://www.w3.org/2000/01/rdf-schema#isDefinedBy> <https://w3id.org/fair/fip/latest/FIP-Question-I2-MD>;
  <http://www.w3.org/2000/01/rdf-schema#label> "FIP Question I2-MD"@en;
  <http://www.w3.org/2004/02/skos/core#definition> "Which structured vocabularies do you use to annotate your metadata records?"@en;
  <https://w3id.org/fair/fip/terms/refers-to-principle> <https://w3id.org/fair/principles/terms/I2> .

<https://w3id.org/fair/fip/terms/FIP-Question-I2-D> a <http://www.w3.org/2002/07/owl#NamedIndividual>,
    <https://w3id.org/fair/fip/terms/FIP-Question>;
  <http://www.w3.org/2000/01/rdf-schema#isDefinedBy> <https://w3id.org/fair/fip/latest/FIP-Question-I2-D>;
  <http://www.w3.org/2000/01/rdf-schema#label> "FIP Question I2-D"@en;
  <http://www.w3.org/2004/02/skos/core#definition> "Which structured vocabularies do you use to encode your datasets?"@en;
  <https://w3id.org/fair/fip/terms/refers-to-principle> <https://w3id.org/fair/principles/terms/I2> .

<https://w3id.org/fair/fip/terms/FIP-Question-I3-MD> a <http://www.w3.org/2002/07/owl#NamedIndividual>,
    <https://w3id.org/fair/fip/terms/FIP-Question>;
  <http://www.w3.org/2000/01/rdf-schema#isDefinedBy> <https://w3id.org/fair/fip/latest/FIP-Question-I3-MD>;
  <http://www.w3.org/2000/01/rdf-schema#label> "FIP Question I3-MD"@en;
  <http://www.w3.org/2004/02/skos/core#definition> "Which models, schema(s) do you use for your metadata records?"@en;
  <https://w3id.org/fair/fip/terms/refers-to-principle> <https://w3id.org/fair/principles/terms/I3> .

<https://w3id.org/fair/fip/terms/FIP-Question-I3-D> a <http://www.w3.org/2002/07/owl#NamedIndividual>,
    <https://w3id.org/fair/fip/terms/FIP-Question>;
  <http://www.w3.org/2000/01/rdf-schema#isDefinedBy> <https://w3id.org/fair/fip/latest/FIP-Question-I3-D>;
  <http://www.w3.org/2000/01/rdf-schema#label> "FIP Question I3-D"@en;
  <http://www.w3.org/2004/02/skos/core#definition> "Which models, schema(s) do you use for your datasets?"@en;
  <https://w3id.org/fair/fip/terms/refers-to-principle> <https://w3id.org/fair/principles/terms/I3> .

<https://w3id.org/fair/fip/terms/FIP-Question-R1.1-MD> a <http://www.w3.org/2002/07/owl#NamedIndividual>,
    <https://w3id.org/fair/fip/terms/FIP-Question>;
  <http://www.w3.org/2000/01/rdf-schema#isDefinedBy> <https://w3id.org/fair/fip/latest/FIP-Question-R1.1-MD>;
  <http://www.w3.org/2000/01/rdf-schema#label> "FIP Question R1.1-MD"@en;
  <http://www.w3.org/2004/02/skos/core#definition> "Which usage license do you use for your metadata records?"@en;
  <https://w3id.org/fair/fip/terms/refers-to-principle> <https://w3id.org/fair/principles/terms/R1.1> .

<https://w3id.org/fair/fip/terms/FIP-Question-R1.1-D> a <http://www.w3.org/2002/07/owl#NamedIndividual>,
    <https://w3id.org/fair/fip/terms/FIP-Question>;
  <http://www.w3.org/2000/01/rdf-schema#isDefinedBy> <https://w3id.org/fair/fip/latest/FIP-Question-R1.1-D>;
  <http://www.w3.org/2000/01/rdf-schema#label> "FIP Question R1.1-D"@en;
  <http://www.w3.org/2004/02/skos/core#definition> "Which usage license do you use for your datasets?"@en;
  <https://w3id.org/fair/fip/terms/refers-to-principle> <https://w3id.org/fair/principles/terms/R1.1> .

<https://w3id.org/fair/fip/terms/FIP-Question-R1.2-MD> a <http://www.w3.org/2002/07/owl#NamedIndividual>,
    <https://w3id.org/fair/fip/terms/FIP-Question>;
  <http://www.w3.org/2000/01/rdf-schema#isDefinedBy> <https://w3id.org/fair/fip/latest/FIP-Question-R1.2-MD>;
  <http://www.w3.org/2000/01/rdf-schema#label> "FIP Question R1.2-MD"@en;
  <http://www.w3.org/2004/02/skos/core#definition> "Which metadata schemas do you use for describing the provenance of your metadata records?"@en;
  <https://w3id.org/fair/fip/terms/refers-to-principle> <https://w3id.org/fair/principles/terms/R1.2> .

<https://w3id.org/fair/fip/terms/FIP-Question-R1.2-D> a <http://www.w3.org/2002/07/owl#NamedIndividual>,
    <https://w3id.org/fair/fip/terms/FIP-Question>;
  <http://www.w3.org/2000/01/rdf-schema#isDefinedBy> <https://w3id.org/fair/fip/latest/FIP-Question-R1.2-D>;
  <http://www.w3.org/2000/01/rdf-schema#label> "FIP Question R1.2-D"@en;
  <http://www.w3.org/2004/02/skos/core#definition> "Which metadata schemas do you use for describing the provenance of your datasets?"@en;
  <https://w3id.org/fair/fip/terms/refers-to-principle> <https://w3id.org/fair/principles/terms/R1.2> .

<https://w3id.org/fair/fip/terms/has-description-source> a <http://www.w3.org/1999/02/22-rdf-syntax-ns#Property>,
    <http://www.w3.org/2002/07/owl#ObjectProperty>;
  <http://www.w3.org/2000/01/rdf-schema#isDefinedBy> <https://w3id.org/fair/fip/latest/has-description-source>;
  <http://www.w3.org/2000/01/rdf-schema#label> "has description source"@en;
  <http://www.w3.org/2004/02/skos/core#definition> "Denotes the source of the description that is asserted via dct:description"@en .

<https://w3id.org/fair/fip/terms/depends-on> a <http://www.w3.org/1999/02/22-rdf-syntax-ns#Property>,
    <http://www.w3.org/2002/07/owl#ObjectProperty>;
  <http://www.w3.org/2000/01/rdf-schema#domain> <https://w3id.org/fair/fip/terms/FAIR-Enabling-Resource>;
  <http://www.w3.org/2000/01/rdf-schema#isDefinedBy> <https://w3id.org/fair/fip/latest/depends-on>;
  <http://www.w3.org/2000/01/rdf-schema#label> "depends on"@en;
  <http://www.w3.org/2000/01/rdf-schema#range> <https://w3id.org/fair/fip/terms/FAIR-Supporting-Software>;
  <http://www.w3.org/2004/02/skos/core#definition> "Connects a FAIR Enabling Resource with a FAIR Supporting Software."@en .

<https://w3id.org/fair/fip/terms/implements> a <http://www.w3.org/1999/02/22-rdf-syntax-ns#Property>,
    <http://www.w3.org/2002/07/owl#ObjectProperty>;
  <http://www.w3.org/2000/01/rdf-schema#domain> <https://w3id.org/fair/fip/terms/FAIR-Enabling-Resource>;
  <http://www.w3.org/2000/01/rdf-schema#isDefinedBy> <https://w3id.org/fair/fip/latest/implements>;
  <http://www.w3.org/2000/01/rdf-schema#label> "implements"@en;
  <http://www.w3.org/2000/01/rdf-schema#range> <https://w3id.org/fair/fip/terms/FAIR-Specification>;
  <http://www.w3.org/2004/02/skos/core#definition> "Connects a FAIR Enabling Resource with a FAIR Specification"@en .

<https://w3id.org/fair/fip/terms/has-data-usage-license> a <http://www.w3.org/1999/02/22-rdf-syntax-ns#Property>,
    <http://www.w3.org/2002/07/owl#ObjectProperty>;
  <http://www.w3.org/2000/01/rdf-schema#domain> <https://w3id.org/fair/fip/terms/FAIR-Enabling-Resource>;
  <http://www.w3.org/2000/01/rdf-schema#isDefinedBy> <https://w3id.org/fair/fip/latest/has-data-usage-license>;
  <http://www.w3.org/2000/01/rdf-schema#label> "has data usage license"@en;
  <http://www.w3.org/2000/01/rdf-schema#range> <https://w3id.org/fair/fip/terms/Data-usage-license>;
  <http://www.w3.org/2004/02/skos/core#definition> "Connects a FAIR Enabling Resource with a data usage license."@en .

<https://w3id.org/fair/fip/terms/has-MPP> a <http://www.w3.org/1999/02/22-rdf-syntax-ns#Property>,
    <http://www.w3.org/2002/07/owl#ObjectProperty>;
  <http://www.w3.org/2000/01/rdf-schema#domain> <https://w3id.org/fair/fip/terms/Registry>;
  <http://www.w3.org/2000/01/rdf-schema#isDefinedBy> <https://w3id.org/fair/fip/latest/has-MPP>;
  <http://www.w3.org/2000/01/rdf-schema#label> "has metadata preservation policy"@en;
  <http://www.w3.org/2000/01/rdf-schema#range> <https://w3id.org/fair/fip/terms/Metadata-preservation-policy>;
  <http://www.w3.org/2004/02/skos/core#definition> "Connects a registry with a metadata preservation policy."@en .

<https://w3id.org/fair/fip/terms/has-AAS> a <http://www.w3.org/1999/02/22-rdf-syntax-ns#Property>,
    <http://www.w3.org/2002/07/owl#ObjectProperty>;
  <http://www.w3.org/2000/01/rdf-schema#domain> <https://w3id.org/fair/fip/terms/Registry>;
  <http://www.w3.org/2000/01/rdf-schema#isDefinedBy> <https://w3id.org/fair/fip/latest/has-AAS>;
  <http://www.w3.org/2000/01/rdf-schema#label> "uses authentication and authorization service"@en;
  <http://www.w3.org/2000/01/rdf-schema#range> <https://w3id.org/fair/fip/terms/Authentication-and-authorization-service>;
  <http://www.w3.org/2004/02/skos/core#definition> "Connects a registry with an authentication and authorization service"@en .

<https://w3id.org/fair/fip/terms/uses-identifier-service> a <http://www.w3.org/1999/02/22-rdf-syntax-ns#Property>,
    <http://www.w3.org/2002/07/owl#ObjectProperty>;
  <http://www.w3.org/2000/01/rdf-schema#domain> <https://w3id.org/fair/fip/terms/Registry>;
  <http://www.w3.org/2000/01/rdf-schema#isDefinedBy> <https://w3id.org/fair/fip/latest/uses-identifier-service>;
  <http://www.w3.org/2000/01/rdf-schema#label> "uses identifier service"@en;
  <http://www.w3.org/2000/01/rdf-schema#range> <https://w3id.org/fair/fip/terms/Identifier-service>;
  <http://www.w3.org/2004/02/skos/core#definition> "Connects a registry with an identifier service."@en .

<https://w3id.org/fair/fip/terms/targets> a <http://www.w3.org/1999/02/22-rdf-syntax-ns#Property>,
    <http://www.w3.org/2002/07/owl#ObjectProperty>;
  <http://www.w3.org/2000/01/rdf-schema#domain> <https://w3id.org/fair/fip/terms/FAIR-Supporting-Resource>;
  <http://www.w3.org/2000/01/rdf-schema#isDefinedBy> <https://w3id.org/fair/fip/latest/targets>;
  <http://www.w3.org/2000/01/rdf-schema#label> "targets"@en;
  <http://www.w3.org/2000/01/rdf-schema#range> <https://w3id.org/fair/fip/terms/Digital-Object-Type>;
  <http://www.w3.org/2004/02/skos/core#definition> "Specifies the type of digital object targeted by a FAIR Supporting Resources"@en .

<https://w3id.org/fair/fip/terms/has-persistency-policy> a <http://www.w3.org/1999/02/22-rdf-syntax-ns#Property>,
    <http://www.w3.org/2002/07/owl#ObjectProperty>;
  <http://www.w3.org/2000/01/rdf-schema#domain> <https://w3id.org/fair/fip/terms/FAIR-Supporting-Resource>;
  <http://www.w3.org/2000/01/rdf-schema#isDefinedBy> <https://w3id.org/fair/fip/latest/has-persistency-policy>;
  <http://www.w3.org/2000/01/rdf-schema#label> "has persistency policy"@en;
  <http://www.w3.org/2000/01/rdf-schema#range> <https://w3id.org/fair/fip/terms/Persistency-Policy>;
  <http://www.w3.org/2004/02/skos/core#definition> "Connects a FAIR Supporting Resource with a persistency policy"@en .

<https://w3id.org/fair/fip/terms/recommended-by> a <http://www.w3.org/1999/02/22-rdf-syntax-ns#Property>,
    <http://www.w3.org/2002/07/owl#ObjectProperty>;
  <http://www.w3.org/2000/01/rdf-schema#domain> <https://w3id.org/fair/fip/terms/FAIR-Supporting-Resource>;
  <http://www.w3.org/2000/01/rdf-schema#isDefinedBy> <https://w3id.org/fair/fip/latest/recommended-by>;
  <http://www.w3.org/2000/01/rdf-schema#label> "is recommended by"@en;
  <http://www.w3.org/2000/01/rdf-schema#range> <https://w3id.org/fair/fip/terms/FAIR-Implementation-Community>;
  <http://www.w3.org/2004/02/skos/core#definition> "Connects a FAIR Supporting Resource with a FAIR Implementation Community that recommends the resource"@en .
