@prefix this: <https://w3id.org/fair/icc/np/FAIR-Principles-Explained-Working-Group/RAMtr_qLjcqCjf_i0y_-OAM1bZdQU8znkKxvnnymovGMs> .
@prefix sub: <https://w3id.org/fair/icc/np/FAIR-Principles-Explained-Working-Group/RAMtr_qLjcqCjf_i0y_-OAM1bZdQU8znkKxvnnymovGMs#> .
@prefix icc: <https://w3id.org/fair/icc/terms/> .
@prefix rdfs: <http://www.w3.org/2000/01/rdf-schema#> .
@prefix xsd: <http://www.w3.org/2001/XMLSchema#> .
@prefix dct: <http://purl.org/dc/terms/> .
@prefix prov: <http://www.w3.org/ns/prov#> .
@prefix np: <http://www.nanopub.org/nschema#> .
@prefix orcid: <https://orcid.org/> .
@prefix foaf: <http://xmlns.com/foaf/0.1/> .

sub:Head {
  this: np:hasAssertion sub:assertion;
    np:hasProvenance sub:provenance;
    np:hasPublicationInfo sub:pubinfo;
    a np:Nanopublication .
}

sub:assertion {
  orcid:0000-0001-5306-5690 rdfs:label "Susanna-Assunta Sansone" .
  
  orcid:0000-0001-6441-6716 rdfs:label "Natalie Meyers" .
  
  orcid:0000-0001-6594-9178 rdfs:label "Christopher Brewster" .
  
  orcid:0000-0001-6960-357X rdfs:label "Mark D. Wilkinson" .
  
  orcid:0000-0001-7030-7030 rdfs:label "Ignasi Labastida" .
  
  orcid:0000-0001-7542-0286 rdfs:label "Egon Willighagen" .
  
  orcid:0000-0001-8414-9272 rdfs:label "Simon Coles" .
  
  orcid:0000-0001-8888-635X rdfs:label "Erik Schultes" .
  
  orcid:0000-0001-9773-4008 rdfs:label "Andra Waagmeester" .
  
  orcid:0000-0001-9853-5668 rdfs:label "Philippe Rocca-Serra" .
  
  orcid:0000-0002-1164-1351 rdfs:label "Luiz Olavo Bonino da Silva Santos" .
  
  orcid:0000-0002-1215-167X rdfs:label "Rajaram Kaliyaperumal" .
  
  orcid:0000-0002-1267-0234 rdfs:label "Tobias Kuhn" .
  
  orcid:0000-0002-1704-5980 rdfs:label "Ronal Cornet" .
  
  orcid:0000-0002-2036-8350 rdfs:label "Nick Juty" .
  
  orcid:0000-0002-3452-553X rdfs:label "Giancarlo Guizzardi" .
  
  orcid:0000-0002-4040-0215 rdfs:label "Tobias Weigel" .
  
  orcid:0000-0002-4182-7560 rdfs:label "Kristina Hettne" .
  
  orcid:0000-0002-4451-8042 rdfs:label "Christine R. Kirkpatrick" .
  
  orcid:0000-0002-5301-3142 rdfs:label "Chris T. Evelo" .
  
  orcid:0000-0002-7633-1442 rdfs:label "Mark Thompson" .
  
  orcid:0000-0002-7641-6446 rdfs:label "Ricardo de Miranda Azevedo" .
  
  orcid:0000-0002-7664-3331 rdfs:label "Juliane Schneider" .
  
  orcid:0000-0002-8042-4131 rdfs:label "Myles Axton" .
  
  orcid:0000-0002-8691-772X rdfs:label "Marco Roos" .
  
  orcid:0000-0002-9551-6370 rdfs:label "MÃ©lanie Courtot" .
  
  orcid:0000-0003-0413-2003 rdfs:label "Annalisa Montesanti" .
  
  orcid:0000-0003-0627-8014 rdfs:label "Mirjam van Reisen" .
  
  orcid:0000-0003-2195-3997 rdfs:label "Barbara Magagna" .
  
  orcid:0000-0003-2376-9755 rdfs:label "Melanie Imming" .
  
  orcid:0000-0003-2687-1982 rdfs:label "Peter McQuilton" .
  
  orcid:0000-0003-2980-4400 rdfs:label "Robert Pergl" .
  
  orcid:0000-0003-3357-3027 rdfs:label "Martijn Kersloot" .
  
  orcid:0000-0003-3538-0106 rdfs:label "Peter Wittenburg" .
  
  orcid:0000-0003-3934-0072 rdfs:label "Barend Mons" .
  
  orcid:0000-0003-4014-4394 rdfs:label "Ali Hasnain" .
  
  orcid:0000-0003-4053-7825 rdfs:label "Keith Jeffery" .
  
  orcid:0000-0003-4098-0464 rdfs:label "George Strawn" .
  
  orcid:0000-0003-4818-2360 rdfs:label "Annika Jacobsen" .
  
  icc:FAIR-Principles-Explained-Working-Group a foaf:Group;
    rdfs:label "FAIR Principles Explained Working Group"@en;
    foaf:member orcid:0000-0001-5306-5690, orcid:0000-0001-6441-6716, orcid:0000-0001-6594-9178,
      orcid:0000-0001-6960-357X, orcid:0000-0001-7030-7030, orcid:0000-0001-7542-0286, orcid:0000-0001-8414-9272,
      orcid:0000-0001-8888-635X, orcid:0000-0001-9773-4008, orcid:0000-0001-9853-5668, orcid:0000-0002-1164-1351,
      orcid:0000-0002-1215-167X, orcid:0000-0002-1267-0234, orcid:0000-0002-1704-5980, orcid:0000-0002-2036-8350,
      orcid:0000-0002-3452-553X, orcid:0000-0002-4040-0215, orcid:0000-0002-4182-7560, orcid:0000-0002-4451-8042,
      orcid:0000-0002-5301-3142, orcid:0000-0002-7633-1442, orcid:0000-0002-7641-6446, orcid:0000-0002-7664-3331,
      orcid:0000-0002-8042-4131, orcid:0000-0002-8691-772X, orcid:0000-0002-9551-6370, orcid:0000-0003-0413-2003,
      orcid:0000-0003-0627-8014, orcid:0000-0003-2195-3997, orcid:0000-0003-2376-9755, orcid:0000-0003-2687-1982,
      orcid:0000-0003-2980-4400, orcid:0000-0003-3357-3027, orcid:0000-0003-3538-0106, orcid:0000-0003-3934-0072,
      orcid:0000-0003-4014-4394, orcid:0000-0003-4053-7825, orcid:0000-0003-4098-0464, orcid:0000-0003-4818-2360 .
}

sub:provenance {
  sub:assertion prov:wasAttributedTo icc:FAIR-Principles-Explained-Working-Group .
}

sub:pubinfo {
  this: dct:created "2019-07-08T14:26:39.208+02:00"^^xsd:dateTime;
    dct:creator orcid:0000-0001-6960-357X, orcid:0000-0002-1267-0234, orcid:0000-0003-4818-2360;
    dct:rights <https://creativecommons.org/publicdomain/zero/1.0> .
}
@prefix this: <https://w3id.org/fair/icc/np/FAIR-ICC-Model/RAO79yJMU83XZbvzo6XFeUpfTFd95q2PxXssSDTI8f2pE> .
@prefix sub: <https://w3id.org/fair/icc/np/FAIR-ICC-Model/RAO79yJMU83XZbvzo6XFeUpfTFd95q2PxXssSDTI8f2pE#> .
@prefix pav: <http://purl.org/pav/> .
@prefix icc: <https://w3id.org/fair/icc/terms/> .
@prefix fair: <https://w3id.org/fair/principles/terms/> .
@prefix np: <http://www.nanopub.org/nschema#> .
@prefix dct: <http://purl.org/dc/terms/> .
@prefix owl: <http://www.w3.org/2002/07/owl#> .
@prefix rdfs: <http://www.w3.org/2000/01/rdf-schema#> .
@prefix xsd: <http://www.w3.org/2001/XMLSchema#> .
@prefix orcid: <https://orcid.org/> .
@prefix vann: <http://purl.org/vocab/vann/> .

sub:Head {
  this: np:hasAssertion sub:assertion;
    np:hasProvenance sub:provenance;
    np:hasPublicationInfo sub:pubinfo;
    a np:Nanopublication .
}

sub:assertion {
  icc:FAIR-ICC-Model dct:creator orcid:0000-0001-6960-357X, orcid:0000-0002-1267-0234,
      orcid:0000-0003-4818-2360;
    dct:description "This is the formal model describing the Implementation Choices and Challenges for the FAIR principles.";
    dct:rights <https://creativecommons.org/publicdomain/zero/1.0/>;
    dct:title "FAIR Implementation Choices and Challenges Model";
    vann:preferredNamespacePrefix "icc";
    vann:preferredNamespaceUri "https://w3id.org/fair/icc/terms/";
    a owl:Ontology;
    rdfs:seeAlso fair:FAIR .
}

sub:provenance {
  sub:assertion pav:authoredBy icc:FAIR-Principles-Explained-Working-Group .
}

sub:pubinfo {
  this: dct:created "2019-07-08T14:26:39.208+02:00"^^xsd:dateTime;
    dct:creator orcid:0000-0001-6960-357X, orcid:0000-0002-1267-0234, orcid:0000-0003-4818-2360;
    dct:license <https://creativecommons.org/publicdomain/zero/1.0/> .
}
@prefix this: <https://w3id.org/fair/icc/np/Consideration/RAQ2XhPvxzFximTOXsTHI3dufKfzNqYe1RajYntET4Miw> .
@prefix sub: <https://w3id.org/fair/icc/np/Consideration/RAQ2XhPvxzFximTOXsTHI3dufKfzNqYe1RajYntET4Miw#> .
@prefix owl: <http://www.w3.org/2002/07/owl#> .
@prefix icc: <https://w3id.org/fair/icc/terms/> .
@prefix rdfs: <http://www.w3.org/2000/01/rdf-schema#> .
@prefix xsd: <http://www.w3.org/2001/XMLSchema#> .
@prefix dct: <http://purl.org/dc/terms/> .
@prefix pav: <http://purl.org/pav/> .
@prefix np: <http://www.nanopub.org/nschema#> .
@prefix orcid: <https://orcid.org/> .
@prefix skos: <http://www.w3.org/2004/02/skos/core#> .

sub:Head {
  this: np:hasAssertion sub:assertion;
    np:hasProvenance sub:provenance;
    np:hasPublicationInfo sub:pubinfo;
    a np:Nanopublication .
}

sub:assertion {
  icc:Consideration a owl:Class;
    rdfs:label "Consideration"@en;
    skos:definition "Something that is either a Choice or a Challenge"@en .
}

sub:provenance {
  sub:assertion pav:authoredBy icc:FAIR-Principles-Explained-Working-Group .
}

sub:pubinfo {
  this: dct:created "2019-07-08T14:26:39.208+02:00"^^xsd:dateTime;
    dct:creator orcid:0000-0001-6960-357X, orcid:0000-0002-1267-0234, orcid:0000-0003-4818-2360;
    dct:license <https://creativecommons.org/publicdomain/zero/1.0/> .
}
@prefix this: <https://w3id.org/fair/icc/np/Choice/RAxgBFasQSBtT7botImkhOcrM0rHluqFzU82nD5ufrgD0> .
@prefix sub: <https://w3id.org/fair/icc/np/Choice/RAxgBFasQSBtT7botImkhOcrM0rHluqFzU82nD5ufrgD0#> .
@prefix icc: <https://w3id.org/fair/icc/terms/> .
@prefix rdfs: <http://www.w3.org/2000/01/rdf-schema#> .
@prefix xsd: <http://www.w3.org/2001/XMLSchema#> .
@prefix dct: <http://purl.org/dc/terms/> .
@prefix pav: <http://purl.org/pav/> .
@prefix np: <http://www.nanopub.org/nschema#> .
@prefix orcid: <https://orcid.org/> .
@prefix skos: <http://www.w3.org/2004/02/skos/core#> .

sub:Head {
  this: np:hasAssertion sub:assertion;
    np:hasProvenance sub:provenance;
    np:hasPublicationInfo sub:pubinfo;
    a np:Nanopublication .
}

sub:assertion {
  icc:Choice rdfs:label "Choice"@en;
    rdfs:subClassOf icc:Consideration;
    skos:definition "The kind of choice communities have to make (can be expressed as a question; choices are represented as rows in the Matrix)"@en .
}

sub:provenance {
  sub:assertion pav:authoredBy icc:FAIR-Principles-Explained-Working-Group .
}

sub:pubinfo {
  this: dct:created "2019-07-08T14:26:39.208+02:00"^^xsd:dateTime;
    dct:creator orcid:0000-0001-6960-357X, orcid:0000-0002-1267-0234, orcid:0000-0003-4818-2360;
    dct:license <https://creativecommons.org/publicdomain/zero/1.0/> .
}
@prefix this: <https://w3id.org/fair/icc/np/Challenge/RAdjhNX-0zQ_HKmj1eVl8ZcJO2qCamqcsMnD_HrIJVH2s> .
@prefix sub: <https://w3id.org/fair/icc/np/Challenge/RAdjhNX-0zQ_HKmj1eVl8ZcJO2qCamqcsMnD_HrIJVH2s#> .
@prefix icc: <https://w3id.org/fair/icc/terms/> .
@prefix rdfs: <http://www.w3.org/2000/01/rdf-schema#> .
@prefix xsd: <http://www.w3.org/2001/XMLSchema#> .
@prefix dct: <http://purl.org/dc/terms/> .
@prefix pav: <http://purl.org/pav/> .
@prefix np: <http://www.nanopub.org/nschema#> .
@prefix orcid: <https://orcid.org/> .
@prefix skos: <http://www.w3.org/2004/02/skos/core#> .

sub:Head {
  this: np:hasAssertion sub:assertion;
    np:hasProvenance sub:provenance;
    np:hasPublicationInfo sub:pubinfo;
    a np:Nanopublication .
}

sub:assertion {
  icc:Challenge rdfs:label "Challenge"@en;
    rdfs:subClassOf icc:Consideration;
    skos:definition "The kind of <strong>challenge</strong> that some communities face if the lack of existing resources doesn't allow them to make a choice yet"@en .
}

sub:provenance {
  sub:assertion pav:authoredBy icc:FAIR-Principles-Explained-Working-Group .
}

sub:pubinfo {
  this: dct:created "2019-07-08T14:26:39.208+02:00"^^xsd:dateTime;
    dct:creator orcid:0000-0001-6960-357X, orcid:0000-0002-1267-0234, orcid:0000-0003-4818-2360;
    dct:license <https://creativecommons.org/publicdomain/zero/1.0/> .
}
@prefix this: <https://w3id.org/fair/icc/np/Declaration/RAUKG4O39QSbjR-PvQYVYmSLInekX1V2x7a10VPfLy7Js> .
@prefix sub: <https://w3id.org/fair/icc/np/Declaration/RAUKG4O39QSbjR-PvQYVYmSLInekX1V2x7a10VPfLy7Js#> .
@prefix owl: <http://www.w3.org/2002/07/owl#> .
@prefix icc: <https://w3id.org/fair/icc/terms/> .
@prefix rdfs: <http://www.w3.org/2000/01/rdf-schema#> .
@prefix xsd: <http://www.w3.org/2001/XMLSchema#> .
@prefix dct: <http://purl.org/dc/terms/> .
@prefix pav: <http://purl.org/pav/> .
@prefix np: <http://www.nanopub.org/nschema#> .
@prefix orcid: <https://orcid.org/> .
@prefix skos: <http://www.w3.org/2004/02/skos/core#> .

sub:Head {
  this: np:hasAssertion sub:assertion;
    np:hasProvenance sub:provenance;
    np:hasPublicationInfo sub:pubinfo;
    a np:Nanopublication .
}

sub:assertion {
  icc:Declaration a owl:Class;
    rdfs:label "Declaration"@en;
    skos:definition "Something that is either a ChoiceDeclaration or a ChallengeDeclaration"@en .
}

sub:provenance {
  sub:assertion pav:authoredBy icc:FAIR-Principles-Explained-Working-Group .
}

sub:pubinfo {
  this: dct:created "2019-07-08T14:26:39.208+02:00"^^xsd:dateTime;
    dct:creator orcid:0000-0001-6960-357X, orcid:0000-0002-1267-0234, orcid:0000-0003-4818-2360;
    dct:license <https://creativecommons.org/publicdomain/zero/1.0/> .
}
@prefix this: <https://w3id.org/fair/icc/np/ChoiceDeclaration/RAWVeAtCZTlSK4H8_d8rdA8-Qtrt0x8WBqQr93wUMD0CM> .
@prefix sub: <https://w3id.org/fair/icc/np/ChoiceDeclaration/RAWVeAtCZTlSK4H8_d8rdA8-Qtrt0x8WBqQr93wUMD0CM#> .
@prefix icc: <https://w3id.org/fair/icc/terms/> .
@prefix rdfs: <http://www.w3.org/2000/01/rdf-schema#> .
@prefix xsd: <http://www.w3.org/2001/XMLSchema#> .
@prefix dct: <http://purl.org/dc/terms/> .
@prefix pav: <http://purl.org/pav/> .
@prefix np: <http://www.nanopub.org/nschema#> .
@prefix orcid: <https://orcid.org/> .
@prefix skos: <http://www.w3.org/2004/02/skos/core#> .

sub:Head {
  this: np:hasAssertion sub:assertion;
    np:hasProvenance sub:provenance;
    np:hasPublicationInfo sub:pubinfo;
    a np:Nanopublication .
}

sub:assertion {
  icc:ChoiceDeclaration rdfs:label "Choice Declaration"@en;
    rdfs:subClassOf icc:Declaration;
    skos:definition "The expression of a community of their choice made (corresponds to an answer to a question, i.e. a cell in the Matrix)"@en .
}

sub:provenance {
  sub:assertion pav:authoredBy icc:FAIR-Principles-Explained-Working-Group .
}

sub:pubinfo {
  this: dct:created "2019-07-08T14:26:39.208+02:00"^^xsd:dateTime;
    dct:creator orcid:0000-0001-6960-357X, orcid:0000-0002-1267-0234, orcid:0000-0003-4818-2360;
    dct:license <https://creativecommons.org/publicdomain/zero/1.0/> .
}
@prefix this: <https://w3id.org/fair/icc/np/ChallengeDeclaration/RAzVGEx1BIdSinmT9JFe4hUXOMbNUCDb7w-O1MJfW4-ow> .
@prefix sub: <https://w3id.org/fair/icc/np/ChallengeDeclaration/RAzVGEx1BIdSinmT9JFe4hUXOMbNUCDb7w-O1MJfW4-ow#> .
@prefix icc: <https://w3id.org/fair/icc/terms/> .
@prefix rdfs: <http://www.w3.org/2000/01/rdf-schema#> .
@prefix xsd: <http://www.w3.org/2001/XMLSchema#> .
@prefix dct: <http://purl.org/dc/terms/> .
@prefix pav: <http://purl.org/pav/> .
@prefix np: <http://www.nanopub.org/nschema#> .
@prefix orcid: <https://orcid.org/> .
@prefix skos: <http://www.w3.org/2004/02/skos/core#> .

sub:Head {
  this: np:hasAssertion sub:assertion;
    np:hasProvenance sub:provenance;
    np:hasPublicationInfo sub:pubinfo;
    a np:Nanopublication .
}

sub:assertion {
  icc:ChallengeDeclaration rdfs:label "Challenge Declaration"@en;
    rdfs:subClassOf icc:Declaration;
    skos:definition "The expression of a community of a challenge they accepted"@en .
}

sub:provenance {
  sub:assertion pav:authoredBy icc:FAIR-Principles-Explained-Working-Group .
}

sub:pubinfo {
  this: dct:created "2019-07-08T14:26:39.208+02:00"^^xsd:dateTime;
    dct:creator orcid:0000-0001-6960-357X, orcid:0000-0002-1267-0234, orcid:0000-0003-4818-2360;
    dct:license <https://creativecommons.org/publicdomain/zero/1.0/> .
}
@prefix this: <https://w3id.org/fair/icc/np/Community/RARtpZ6XN0M-WXmCvmXbqzGq7EZiRViy27c0_Kg7L8qbQ> .
@prefix sub: <https://w3id.org/fair/icc/np/Community/RARtpZ6XN0M-WXmCvmXbqzGq7EZiRViy27c0_Kg7L8qbQ#> .
@prefix owl: <http://www.w3.org/2002/07/owl#> .
@prefix icc: <https://w3id.org/fair/icc/terms/> .
@prefix rdfs: <http://www.w3.org/2000/01/rdf-schema#> .
@prefix xsd: <http://www.w3.org/2001/XMLSchema#> .
@prefix dct: <http://purl.org/dc/terms/> .
@prefix pav: <http://purl.org/pav/> .
@prefix np: <http://www.nanopub.org/nschema#> .
@prefix orcid: <https://orcid.org/> .
@prefix skos: <http://www.w3.org/2004/02/skos/core#> .

sub:Head {
  this: np:hasAssertion sub:assertion;
    np:hasProvenance sub:provenance;
    np:hasPublicationInfo sub:pubinfo;
    a np:Nanopublication .
}

sub:assertion {
  icc:Community a owl:Class;
    rdfs:label "Community"@en;
    skos:definition "A non-empty set of people and/or organizations that form a self-declared community with the aim to implement the FAIR principles for their fields of interest (communities are represented as columns in the Matrix)"@en .
}

sub:provenance {
  sub:assertion pav:authoredBy icc:FAIR-Principles-Explained-Working-Group .
}

sub:pubinfo {
  this: dct:created "2019-07-08T14:26:39.208+02:00"^^xsd:dateTime;
    dct:creator orcid:0000-0001-6960-357X, orcid:0000-0002-1267-0234, orcid:0000-0003-4818-2360;
    dct:license <https://creativecommons.org/publicdomain/zero/1.0/> .
}
@prefix this: <https://w3id.org/fair/icc/np/Resource/RA9Tc6QNK5y22ylB0dVpKB3GiyhfThlLa0C2Gmexnb5_s> .
@prefix sub: <https://w3id.org/fair/icc/np/Resource/RA9Tc6QNK5y22ylB0dVpKB3GiyhfThlLa0C2Gmexnb5_s#> .
@prefix owl: <http://www.w3.org/2002/07/owl#> .
@prefix icc: <https://w3id.org/fair/icc/terms/> .
@prefix rdfs: <http://www.w3.org/2000/01/rdf-schema#> .
@prefix xsd: <http://www.w3.org/2001/XMLSchema#> .
@prefix dct: <http://purl.org/dc/terms/> .
@prefix pav: <http://purl.org/pav/> .
@prefix np: <http://www.nanopub.org/nschema#> .
@prefix orcid: <https://orcid.org/> .
@prefix skos: <http://www.w3.org/2004/02/skos/core#> .

sub:Head {
  this: np:hasAssertion sub:assertion;
    np:hasProvenance sub:provenance;
    np:hasPublicationInfo sub:pubinfo;
    a np:Nanopublication .
}

sub:assertion {
  icc:Resource a owl:Class;
    rdfs:label "Resource"@en;
    skos:definition "An artifact or service that can contribute to the implementation of the FAIR principles (corresponds to the possible values of the cells in the Matrix)"@en .
}

sub:provenance {
  sub:assertion pav:authoredBy icc:FAIR-Principles-Explained-Working-Group .
}

sub:pubinfo {
  this: dct:created "2019-07-08T14:26:39.208+02:00"^^xsd:dateTime;
    dct:creator orcid:0000-0001-6960-357X, orcid:0000-0002-1267-0234, orcid:0000-0003-4818-2360;
    dct:license <https://creativecommons.org/publicdomain/zero/1.0/> .
}
@prefix this: <https://w3id.org/fair/icc/np/Explanation/RAolWD1jRbr8pBBgfC_MScNiOXcyAQnwJqH0J6Ig4DkVs> .
@prefix sub: <https://w3id.org/fair/icc/np/Explanation/RAolWD1jRbr8pBBgfC_MScNiOXcyAQnwJqH0J6Ig4DkVs#> .
@prefix owl: <http://www.w3.org/2002/07/owl#> .
@prefix icc: <https://w3id.org/fair/icc/terms/> .
@prefix rdfs: <http://www.w3.org/2000/01/rdf-schema#> .
@prefix xsd: <http://www.w3.org/2001/XMLSchema#> .
@prefix dct: <http://purl.org/dc/terms/> .
@prefix pav: <http://purl.org/pav/> .
@prefix np: <http://www.nanopub.org/nschema#> .
@prefix orcid: <https://orcid.org/> .
@prefix skos: <http://www.w3.org/2004/02/skos/core#> .

sub:Head {
  this: np:hasAssertion sub:assertion;
    np:hasProvenance sub:provenance;
    np:hasPublicationInfo sub:pubinfo;
    a np:Nanopublication .
}

sub:assertion {
  icc:Explanation a owl:Class;
    rdfs:label "Explanation"@en;
    skos:definition "An explanation of a FAIR (sub)principle"@en .
}

sub:provenance {
  sub:assertion pav:authoredBy icc:FAIR-Principles-Explained-Working-Group .
}

sub:pubinfo {
  this: dct:created "2019-07-08T14:26:39.208+02:00"^^xsd:dateTime;
    dct:creator orcid:0000-0001-6960-357X, orcid:0000-0002-1267-0234, orcid:0000-0003-4818-2360;
    dct:license <https://creativecommons.org/publicdomain/zero/1.0/> .
}
@prefix this: <https://w3id.org/fair/icc/np/explains-principle/RAan-8B12Hs2XDopx4WrM2KGKpUkQqyAu0K_XaSKTEdPM> .
@prefix sub: <https://w3id.org/fair/icc/np/explains-principle/RAan-8B12Hs2XDopx4WrM2KGKpUkQqyAu0K_XaSKTEdPM#> .
@prefix icc: <https://w3id.org/fair/icc/terms/> .
@prefix fair: <https://w3id.org/fair/principles/terms/> .
@prefix rdf: <http://www.w3.org/1999/02/22-rdf-syntax-ns#> .
@prefix rdfs: <http://www.w3.org/2000/01/rdf-schema#> .
@prefix xsd: <http://www.w3.org/2001/XMLSchema#> .
@prefix dct: <http://purl.org/dc/terms/> .
@prefix pav: <http://purl.org/pav/> .
@prefix np: <http://www.nanopub.org/nschema#> .
@prefix orcid: <https://orcid.org/> .
@prefix skos: <http://www.w3.org/2004/02/skos/core#> .

sub:Head {
  this: np:hasAssertion sub:assertion;
    np:hasProvenance sub:provenance;
    np:hasPublicationInfo sub:pubinfo;
    a np:Nanopublication .
}

sub:assertion {
  icc:explains-principle a rdf:Property;
    rdfs:domain icc:Explanation;
    rdfs:label "explains principle"@en;
    rdfs:range fair:FAIR-Principle-or-SubPrinciple;
    skos:definition "Links an explanation to the FAIR (sub)principle it explains"@en .
}

sub:provenance {
  sub:assertion pav:authoredBy icc:FAIR-Principles-Explained-Working-Group .
}

sub:pubinfo {
  this: dct:created "2019-07-08T14:26:39.208+02:00"^^xsd:dateTime;
    dct:creator orcid:0000-0001-6960-357X, orcid:0000-0002-1267-0234, orcid:0000-0003-4818-2360;
    dct:license <https://creativecommons.org/publicdomain/zero/1.0/> .
}
@prefix this: <https://w3id.org/fair/icc/np/refers-to-principle/RAz6HxZKZBce4C2pw6MskA04XPSMdRJovaelJt_jTtmvM> .
@prefix sub: <https://w3id.org/fair/icc/np/refers-to-principle/RAz6HxZKZBce4C2pw6MskA04XPSMdRJovaelJt_jTtmvM#> .
@prefix icc: <https://w3id.org/fair/icc/terms/> .
@prefix fair: <https://w3id.org/fair/principles/terms/> .
@prefix rdf: <http://www.w3.org/1999/02/22-rdf-syntax-ns#> .
@prefix rdfs: <http://www.w3.org/2000/01/rdf-schema#> .
@prefix xsd: <http://www.w3.org/2001/XMLSchema#> .
@prefix dct: <http://purl.org/dc/terms/> .
@prefix pav: <http://purl.org/pav/> .
@prefix np: <http://www.nanopub.org/nschema#> .
@prefix orcid: <https://orcid.org/> .
@prefix skos: <http://www.w3.org/2004/02/skos/core#> .

sub:Head {
  this: np:hasAssertion sub:assertion;
    np:hasProvenance sub:provenance;
    np:hasPublicationInfo sub:pubinfo;
    a np:Nanopublication .
}

sub:assertion {
  icc:refers-to-principle a rdf:Property;
    rdfs:domain icc:Consideration;
    rdfs:label "refers to principle"@en;
    rdfs:range fair:FAIR-Principle-or-SubPrinciple;
    skos:definition "Connects a Consideration to a FAIR (sub)principle it refers to"@en .
}

sub:provenance {
  sub:assertion pav:authoredBy icc:FAIR-Principles-Explained-Working-Group .
}

sub:pubinfo {
  this: dct:created "2019-07-08T14:26:39.208+02:00"^^xsd:dateTime;
    dct:creator orcid:0000-0001-6960-357X, orcid:0000-0002-1267-0234, orcid:0000-0003-4818-2360;
    dct:license <https://creativecommons.org/publicdomain/zero/1.0/> .
}
@prefix this: <https://w3id.org/fair/icc/np/related-challenge/RAoGLkTg_20RwxCAeOsBUuBQ9BNLObsongWmrG9C3Dvc8> .
@prefix sub: <https://w3id.org/fair/icc/np/related-challenge/RAoGLkTg_20RwxCAeOsBUuBQ9BNLObsongWmrG9C3Dvc8#> .
@prefix icc: <https://w3id.org/fair/icc/terms/> .
@prefix rdf: <http://www.w3.org/1999/02/22-rdf-syntax-ns#> .
@prefix rdfs: <http://www.w3.org/2000/01/rdf-schema#> .
@prefix xsd: <http://www.w3.org/2001/XMLSchema#> .
@prefix dct: <http://purl.org/dc/terms/> .
@prefix pav: <http://purl.org/pav/> .
@prefix np: <http://www.nanopub.org/nschema#> .
@prefix orcid: <https://orcid.org/> .
@prefix skos: <http://www.w3.org/2004/02/skos/core#> .

sub:Head {
  this: np:hasAssertion sub:assertion;
    np:hasProvenance sub:provenance;
    np:hasPublicationInfo sub:pubinfo;
    a np:Nanopublication .
}

sub:assertion {
  icc:related-challenge a rdf:Property;
    rdfs:domain icc:Choice;
    rdfs:label "related challenge"@en;
    rdfs:range icc:Challenge;
    skos:definition "Connects a Choice to a Challenge that some communities might face before they can make the given kind of choice"@en .
}

sub:provenance {
  sub:assertion pav:authoredBy icc:FAIR-Principles-Explained-Working-Group .
}

sub:pubinfo {
  this: dct:created "2019-07-08T14:26:39.208+02:00"^^xsd:dateTime;
    dct:creator orcid:0000-0001-6960-357X, orcid:0000-0002-1267-0234, orcid:0000-0003-4818-2360;
    dct:license <https://creativecommons.org/publicdomain/zero/1.0/> .
}
@prefix this: <https://w3id.org/fair/icc/np/refers-to-consideration/RAZB9xQ4YFUXA2uVAIW38nmsEi3UKENxhkdrFs6Fb0x0c> .
@prefix sub: <https://w3id.org/fair/icc/np/refers-to-consideration/RAZB9xQ4YFUXA2uVAIW38nmsEi3UKENxhkdrFs6Fb0x0c#> .
@prefix icc: <https://w3id.org/fair/icc/terms/> .
@prefix rdf: <http://www.w3.org/1999/02/22-rdf-syntax-ns#> .
@prefix rdfs: <http://www.w3.org/2000/01/rdf-schema#> .
@prefix xsd: <http://www.w3.org/2001/XMLSchema#> .
@prefix dct: <http://purl.org/dc/terms/> .
@prefix pav: <http://purl.org/pav/> .
@prefix np: <http://www.nanopub.org/nschema#> .
@prefix orcid: <https://orcid.org/> .
@prefix skos: <http://www.w3.org/2004/02/skos/core#> .

sub:Head {
  this: np:hasAssertion sub:assertion;
    np:hasProvenance sub:provenance;
    np:hasPublicationInfo sub:pubinfo;
    a np:Nanopublication .
}

sub:assertion {
  icc:refers-to-consideration a rdf:Property;
    rdfs:domain icc:Declaration;
    rdfs:label "refers to consideration"@en;
    rdfs:range icc:Consideration;
    skos:definition "Connects a Declaration to the Consideration it is derived from (indicates row of the Matrix for choice declarations)"@en .
}

sub:provenance {
  sub:assertion pav:authoredBy icc:FAIR-Principles-Explained-Working-Group .
}

sub:pubinfo {
  this: dct:created "2019-07-08T14:26:39.208+02:00"^^xsd:dateTime;
    dct:creator orcid:0000-0001-6960-357X, orcid:0000-0002-1267-0234, orcid:0000-0003-4818-2360;
    dct:license <https://creativecommons.org/publicdomain/zero/1.0/> .
}
@prefix this: <https://w3id.org/fair/icc/np/declared-by/RAE9Kio-8HF1bVeyp7aYw6H2RvocPtOWetDtW0pJQpBQI> .
@prefix sub: <https://w3id.org/fair/icc/np/declared-by/RAE9Kio-8HF1bVeyp7aYw6H2RvocPtOWetDtW0pJQpBQI#> .
@prefix icc: <https://w3id.org/fair/icc/terms/> .
@prefix rdf: <http://www.w3.org/1999/02/22-rdf-syntax-ns#> .
@prefix rdfs: <http://www.w3.org/2000/01/rdf-schema#> .
@prefix xsd: <http://www.w3.org/2001/XMLSchema#> .
@prefix dct: <http://purl.org/dc/terms/> .
@prefix pav: <http://purl.org/pav/> .
@prefix np: <http://www.nanopub.org/nschema#> .
@prefix orcid: <https://orcid.org/> .
@prefix skos: <http://www.w3.org/2004/02/skos/core#> .

sub:Head {
  this: np:hasAssertion sub:assertion;
    np:hasProvenance sub:provenance;
    np:hasPublicationInfo sub:pubinfo;
    a np:Nanopublication .
}

sub:assertion {
  icc:declared-by a rdf:Property;
    rdfs:domain icc:Declaration;
    rdfs:label "declared by"@en;
    rdfs:range icc:Community;
    skos:definition "Connects a Declaration to the Community that made the declaration"@en .
}

sub:provenance {
  sub:assertion pav:authoredBy icc:FAIR-Principles-Explained-Working-Group .
}

sub:pubinfo {
  this: dct:created "2019-07-08T14:26:39.208+02:00"^^xsd:dateTime;
    dct:creator orcid:0000-0001-6960-357X, orcid:0000-0002-1267-0234, orcid:0000-0003-4818-2360;
    dct:license <https://creativecommons.org/publicdomain/zero/1.0/> .
}
@prefix this: <https://w3id.org/fair/icc/np/chosen-resource/RAoztoqSAq44jrgs6-i1hu_kE-Y9AqDM6s0uR2YIpuUl4> .
@prefix sub: <https://w3id.org/fair/icc/np/chosen-resource/RAoztoqSAq44jrgs6-i1hu_kE-Y9AqDM6s0uR2YIpuUl4#> .
@prefix icc: <https://w3id.org/fair/icc/terms/> .
@prefix rdf: <http://www.w3.org/1999/02/22-rdf-syntax-ns#> .
@prefix rdfs: <http://www.w3.org/2000/01/rdf-schema#> .
@prefix xsd: <http://www.w3.org/2001/XMLSchema#> .
@prefix dct: <http://purl.org/dc/terms/> .
@prefix pav: <http://purl.org/pav/> .
@prefix np: <http://www.nanopub.org/nschema#> .
@prefix orcid: <https://orcid.org/> .
@prefix skos: <http://www.w3.org/2004/02/skos/core#> .

sub:Head {
  this: np:hasAssertion sub:assertion;
    np:hasProvenance sub:provenance;
    np:hasPublicationInfo sub:pubinfo;
    a np:Nanopublication .
}

sub:assertion {
  icc:chosen-resource a rdf:Property;
    rdfs:domain icc:ChoiceDeclaration;
    rdfs:label "chosen resource"@en;
    rdfs:range icc:Resource;
    skos:definition "Connects ChoiceDeclaration to the Resource that was chosen through the declaration"@en .
}

sub:provenance {
  sub:assertion pav:authoredBy icc:FAIR-Principles-Explained-Working-Group .
}

sub:pubinfo {
  this: dct:created "2019-07-08T14:26:39.208+02:00"^^xsd:dateTime;
    dct:creator orcid:0000-0001-6960-357X, orcid:0000-0002-1267-0234, orcid:0000-0003-4818-2360;
    dct:license <https://creativecommons.org/publicdomain/zero/1.0/> .
}
@prefix this: <https://w3id.org/fair/icc/np/has-open-challenge/RAqZdSGp7lji61Ktn1-tElQ404POzdVx_ItUqblBjTf3s> .
@prefix sub: <https://w3id.org/fair/icc/np/has-open-challenge/RAqZdSGp7lji61Ktn1-tElQ404POzdVx_ItUqblBjTf3s#> .
@prefix icc: <https://w3id.org/fair/icc/terms/> .
@prefix rdf: <http://www.w3.org/1999/02/22-rdf-syntax-ns#> .
@prefix rdfs: <http://www.w3.org/2000/01/rdf-schema#> .
@prefix xsd: <http://www.w3.org/2001/XMLSchema#> .
@prefix dct: <http://purl.org/dc/terms/> .
@prefix pav: <http://purl.org/pav/> .
@prefix np: <http://www.nanopub.org/nschema#> .
@prefix orcid: <https://orcid.org/> .
@prefix skos: <http://www.w3.org/2004/02/skos/core#> .

sub:Head {
  this: np:hasAssertion sub:assertion;
    np:hasProvenance sub:provenance;
    np:hasPublicationInfo sub:pubinfo;
    a np:Nanopublication .
}

sub:assertion {
  icc:has-open-challenge a rdf:Property;
    rdfs:domain icc:ChoiceDeclaration;
    rdfs:label "has open challenge"@en;
    rdfs:range icc:ChallengeDeclaration;
    skos:definition "Connects a ChoiceDeclaration that doesn't have a chosen resource to a ChallengeDeclaration that describes a challenge that has to be met before the community can choose a resource"@en .
}

sub:provenance {
  sub:assertion pav:authoredBy icc:FAIR-Principles-Explained-Working-Group .
}

sub:pubinfo {
  this: dct:created "2019-07-08T14:26:39.208+02:00"^^xsd:dateTime;
    dct:creator orcid:0000-0001-6960-357X, orcid:0000-0002-1267-0234, orcid:0000-0003-4818-2360;
    dct:license <https://creativecommons.org/publicdomain/zero/1.0/> .
}
@prefix this: <https://w3id.org/fair/icc/np/F1-Explanation/RAqrEnmOe8gCcPPJijCdGTSoN4svEl67hpgLaRlWP7b28> .
@prefix sub: <https://w3id.org/fair/icc/np/F1-Explanation/RAqrEnmOe8gCcPPJijCdGTSoN4svEl67hpgLaRlWP7b28#> .
@prefix icc: <https://w3id.org/fair/icc/terms/> .
@prefix fair: <https://w3id.org/fair/principles/terms/> .
@prefix rdfs: <http://www.w3.org/2000/01/rdf-schema#> .
@prefix xsd: <http://www.w3.org/2001/XMLSchema#> .
@prefix dct: <http://purl.org/dc/terms/> .
@prefix pav: <http://purl.org/pav/> .
@prefix np: <http://www.nanopub.org/nschema#> .
@prefix orcid: <https://orcid.org/> .

sub:Head {
  this: np:hasAssertion sub:assertion;
    np:hasProvenance sub:provenance;
    np:hasPublicationInfo sub:pubinfo;
    a np:Nanopublication .
}

sub:assertion {
  icc:F1-Explanation a icc:Explanation;
    rdfs:comment "Principle F1 states that resources, i.e. data and metadata, should be assigned a globally unique and persistent identifier (GUPID). ...";
    rdfs:label "F1 Explanation";
    icc:explains-principle fair:F1 .
}

sub:provenance {
  sub:assertion pav:authoredBy icc:FAIR-Principles-Explained-Working-Group .
}

sub:pubinfo {
  this: dct:created "2019-07-08T14:26:39.208+02:00"^^xsd:dateTime;
    dct:creator orcid:0000-0001-6960-357X, orcid:0000-0002-1267-0234, orcid:0000-0003-4818-2360;
    dct:license <https://creativecommons.org/publicdomain/zero/1.0/> .
}
@prefix this: <https://w3id.org/fair/icc/np/A1.1-Explanation/RA9qDwvjqppPfzcmpbe6343nYesVd-h0HRtjAtn1NR5X0> .
@prefix sub: <https://w3id.org/fair/icc/np/A1.1-Explanation/RA9qDwvjqppPfzcmpbe6343nYesVd-h0HRtjAtn1NR5X0#> .
@prefix icc: <https://w3id.org/fair/icc/terms/> .
@prefix fair: <https://w3id.org/fair/principles/terms/> .
@prefix rdfs: <http://www.w3.org/2000/01/rdf-schema#> .
@prefix xsd: <http://www.w3.org/2001/XMLSchema#> .
@prefix dct: <http://purl.org/dc/terms/> .
@prefix pav: <http://purl.org/pav/> .
@prefix np: <http://www.nanopub.org/nschema#> .
@prefix orcid: <https://orcid.org/> .

sub:Head {
  this: np:hasAssertion sub:assertion;
    np:hasProvenance sub:provenance;
    np:hasPublicationInfo sub:pubinfo;
    a np:Nanopublication .
}

sub:assertion {
  icc:A1.1-Explanation a icc:Explanation;
    rdfs:comment "With the advent of the World Wide Web, based on open, free, and standardised communication protocols, reduce the cost of gaining access to digital resources. Having a protocol that is open allows any individual to create their own standard-compliant implementation, that it is free reduces the possibility that those lacking monetary means cannot access the resource, and that it is universally implementable ensures that such technology is available to all (and not restricted, for instance by country or creed).";
    rdfs:label "A1.1 Explanation";
    icc:explains-principle fair:A1.1 .
}

sub:provenance {
  sub:assertion pav:authoredBy icc:FAIR-Principles-Explained-Working-Group .
}

sub:pubinfo {
  this: dct:created "2019-07-08T14:26:39.208+02:00"^^xsd:dateTime;
    dct:creator orcid:0000-0001-6960-357X, orcid:0000-0002-1267-0234, orcid:0000-0003-4818-2360;
    dct:license <https://creativecommons.org/publicdomain/zero/1.0/> .
}
@prefix this: <https://w3id.org/fair/icc/np/A1.2-Explanation/RAQVc2HiZGG30zGd9OZfBxz33p8buCkv2oL-ZRIkayZz0> .
@prefix sub: <https://w3id.org/fair/icc/np/A1.2-Explanation/RAQVc2HiZGG30zGd9OZfBxz33p8buCkv2oL-ZRIkayZz0#> .
@prefix icc: <https://w3id.org/fair/icc/terms/> .
@prefix fair: <https://w3id.org/fair/principles/terms/> .
@prefix rdfs: <http://www.w3.org/2000/01/rdf-schema#> .
@prefix xsd: <http://www.w3.org/2001/XMLSchema#> .
@prefix dct: <http://purl.org/dc/terms/> .
@prefix pav: <http://purl.org/pav/> .
@prefix np: <http://www.nanopub.org/nschema#> .
@prefix orcid: <https://orcid.org/> .

sub:Head {
  this: np:hasAssertion sub:assertion;
    np:hasProvenance sub:provenance;
    np:hasPublicationInfo sub:pubinfo;
    a np:Nanopublication .
}

sub:assertion {
  icc:A1.2-Explanation a icc:Explanation;
    rdfs:comment "Some digital resources, such as sensitive individual data, require additional measures to be followed, such as ethical approval, before access can be granted. The âAâ in FAIR does not imply âOpenâ or âFreeâ, but it does require that the exact conditions and the process to access restricted data are transparent and made public. Any additional authentication and authorization procedures must be specified. Therefore, prior to the release of a restricted digital resource, publishers must take steps to clarify eligibility and process.";
    rdfs:label "A1.2 Explanation";
    icc:explains-principle fair:A1.2 .
}

sub:provenance {
  sub:assertion pav:authoredBy icc:FAIR-Principles-Explained-Working-Group .
}

sub:pubinfo {
  this: dct:created "2019-07-08T14:26:39.208+02:00"^^xsd:dateTime;
    dct:creator orcid:0000-0001-6960-357X, orcid:0000-0002-1267-0234, orcid:0000-0003-4818-2360;
    dct:license <https://creativecommons.org/publicdomain/zero/1.0/> .
}
@prefix this: <https://w3id.org/fair/icc/np/A1-Explanation/RA24E0Yzz42puSIwJNgguzpF8ju513jnKNeW17SoTUNCc> .
@prefix sub: <https://w3id.org/fair/icc/np/A1-Explanation/RA24E0Yzz42puSIwJNgguzpF8ju513jnKNeW17SoTUNCc#> .
@prefix icc: <https://w3id.org/fair/icc/terms/> .
@prefix fair: <https://w3id.org/fair/principles/terms/> .
@prefix rdfs: <http://www.w3.org/2000/01/rdf-schema#> .
@prefix xsd: <http://www.w3.org/2001/XMLSchema#> .
@prefix dct: <http://purl.org/dc/terms/> .
@prefix pav: <http://purl.org/pav/> .
@prefix np: <http://www.nanopub.org/nschema#> .
@prefix orcid: <https://orcid.org/> .

sub:Head {
  this: np:hasAssertion sub:assertion;
    np:hasProvenance sub:provenance;
    np:hasPublicationInfo sub:pubinfo;
    a np:Nanopublication .
}

sub:assertion {
  icc:A1-Explanation a icc:Explanation;
    rdfs:comment "FAIR resources and their metadata should be retrievable  using their identifiers in combination with standardised communication protocols. Conditions of compliance are further specified in sub-principles A1.1 and A1.2. ...";
    rdfs:label "A1 Explanation";
    rdfs:seeAlso icc:A1.1-Explanation, icc:A1.2-Explanation;
    icc:explains-principle fair:A1 .
}

sub:provenance {
  sub:assertion pav:authoredBy icc:FAIR-Principles-Explained-Working-Group .
}

sub:pubinfo {
  this: dct:created "2019-07-08T14:26:39.208+02:00"^^xsd:dateTime;
    dct:creator orcid:0000-0001-6960-357X, orcid:0000-0002-1267-0234, orcid:0000-0003-4818-2360;
    dct:license <https://creativecommons.org/publicdomain/zero/1.0/> .
}
@prefix this: <https://w3id.org/fair/icc/np/ICC1/RAvGHtTcgzSjjiuJzfk7ay8TFeIYb63ZRBGVPI1fc9IsQ> .
@prefix sub: <https://w3id.org/fair/icc/np/ICC1/RAvGHtTcgzSjjiuJzfk7ay8TFeIYb63ZRBGVPI1fc9IsQ#> .
@prefix rdfs: <http://www.w3.org/2000/01/rdf-schema#> .
@prefix icc: <https://w3id.org/fair/icc/terms/> .
@prefix fair: <https://w3id.org/fair/principles/terms/> .
@prefix xsd: <http://www.w3.org/2001/XMLSchema#> .
@prefix dct: <http://purl.org/dc/terms/> .
@prefix pav: <http://purl.org/pav/> .
@prefix np: <http://www.nanopub.org/nschema#> .
@prefix orcid: <https://orcid.org/> .

sub:Head {
  this: np:hasAssertion sub:assertion;
    np:hasProvenance sub:provenance;
    np:hasPublicationInfo sub:pubinfo;
    a np:Nanopublication .
}

sub:assertion {
  icc:F1-Challenge-1 a icc:Challenge;
    rdfs:comment "The community should define identifier registration service(s) that ensure global uniqueness for its digital resources.";
    rdfs:label "F1 Challenge 1";
    rdfs:seeAlso icc:F1-Explanation;
    icc:refers-to-principle fair:F1 .
  
  icc:F1-Choice a icc:Choice;
    rdfs:comment "The community should choose identifier registration service(s) that ensure global uniqueness for its digital resources.";
    rdfs:label "F1 Choice";
    rdfs:seeAlso icc:F1-Explanation;
    icc:refers-to-principle fair:F1;
    icc:related-challenge icc:F1-Challenge-1 .
}

sub:provenance {
  sub:assertion pav:authoredBy icc:FAIR-Principles-Explained-Working-Group .
}

sub:pubinfo {
  this: dct:created "2019-07-08T14:26:39.208+02:00"^^xsd:dateTime;
    dct:creator orcid:0000-0001-6960-357X, orcid:0000-0002-1267-0234, orcid:0000-0003-4818-2360;
    dct:license <https://creativecommons.org/publicdomain/zero/1.0/> .
}
