@prefix : <https://w3id.org/fair/fip/terms/FIP-Ontology#> .
@prefix owl: <http://www.w3.org/2002/07/owl#> .
@prefix rdf: <http://www.w3.org/1999/02/22-rdf-syntax-ns#> .
@prefix xml: <http://www.w3.org/XML/1998/namespace> .
@prefix xsd: <http://www.w3.org/2001/XMLSchema#> .
@prefix rdfs: <http://www.w3.org/2000/01/rdf-schema#> .
@base <https://w3id.org/fair/fip/terms/FIP-Ontology> .

<https://w3id.org/fair/fip/terms/FIP-Ontology> rdf:type owl:Ontology ;
                                                <http://purl.org/dc/terms/creator> <https://orcid.org/0000-0001-8888-635X> ,
                                                                                   <https://orcid.org/0000-0002-1267-0234> ,
                                                                                   <https://orcid.org/0000-0003-2195-3997> ;
                                                <http://purl.org/dc/terms/description> "This is an ontology of the FAIR Implementation Profiles (FIP) for the FAIR principles." ;
                                                <http://purl.org/dc/terms/license> <https://creativecommons.org/publicdomain/zero/1.0/> ;
                                                <http://purl.org/dc/terms/title> "FAIR Implementation Profile (FIP) Ontology" ;
                                                <http://purl.org/vocab/vann/preferredNamespacePrefix> "fip" ;
                                                <http://purl.org/vocab/vann/preferredNamespaceUri> "https://w3id.org/fair/fip/terms/" ;
                                                rdfs:isDefinedBy <https://w3id.org/fair/fip/latest/FIP-Ontology> ;
                                                rdfs:seeAlso <https://w3id.org/fair/principles/terms/FAIR> .

#################################################################
#    Annotation properties
#################################################################

###  http://purl.org/dc/terms/creator
<http://purl.org/dc/terms/creator> rdf:type owl:AnnotationProperty .


###  http://purl.org/dc/terms/description
<http://purl.org/dc/terms/description> rdf:type owl:AnnotationProperty .


###  http://purl.org/dc/terms/license
<http://purl.org/dc/terms/license> rdf:type owl:AnnotationProperty .


###  http://purl.org/dc/terms/title
<http://purl.org/dc/terms/title> rdf:type owl:AnnotationProperty .


###  http://purl.org/vocab/vann/preferredNamespacePrefix
<http://purl.org/vocab/vann/preferredNamespacePrefix> rdf:type owl:AnnotationProperty .


###  http://purl.org/vocab/vann/preferredNamespaceUri
<http://purl.org/vocab/vann/preferredNamespaceUri> rdf:type owl:AnnotationProperty .


###  http://www.w3.org/2004/02/skos/core#definition
<http://www.w3.org/2004/02/skos/core#definition> rdf:type owl:AnnotationProperty .


#################################################################
#    Object Properties
#################################################################

###  http://www.w3.org/2000/01/rdf-schema#seeAlso
rdfs:seeAlso rdf:type owl:ObjectProperty .


###  http://xmlns.com/foaf/0.1/member
<http://xmlns.com/foaf/0.1/member> rdf:type owl:ObjectProperty .


###  https://w3id.org/fair/fip/terms/declared-by
<https://w3id.org/fair/fip/terms/declared-by> rdf:type owl:ObjectProperty ;
                                              rdfs:domain <https://w3id.org/fair/fip/terms/FAIR-Declaration> ;
                                              rdfs:range <https://w3id.org/fair/fip/terms/FAIR-Implementation-Community> ;
                                              rdfs:isDefinedBy <https://w3id.org/fair/fip/latest/declared-by> ;
                                              rdfs:label "declared by"@en ;
                                              <http://www.w3.org/2004/02/skos/core#definition> "Connects a FIP declaration to the community that made the declaration"@en .


###  https://w3id.org/fair/fip/terms/declared-for-case-study
<https://w3id.org/fair/fip/terms/declared-for-case-study> rdf:type owl:ObjectProperty ;
                                                          rdfs:domain <https://w3id.org/fair/fip/terms/FAIR-Declaration> ;
                                                          rdfs:range <https://w3id.org/fair/fip/terms/FAIR-Case-Study> ;
                                                          rdfs:isDefinedBy <https://w3id.org/fair/fip/latest/declared-for-case-study> ;
                                                          rdfs:label "declared for case study"@en ;
                                                          <http://www.w3.org/2004/02/skos/core#definition> "Connects a FIP declaration to the case study it refers to."@en .


###  https://w3id.org/fair/fip/terms/declared-for-digital-object-type
<https://w3id.org/fair/fip/terms/declared-for-digital-object-type> rdf:type owl:ObjectProperty ;
                                                                   rdfs:domain <https://w3id.org/fair/fip/terms/FAIR-Declaration> ;
                                                                   rdfs:range <https://w3id.org/fair/fip/terms/Digital-Object-Type> ;
                                                                   rdfs:isDefinedBy <https://w3id.org/fair/fip/latest/declared-for-digital-object-type> ;
                                                                   rdfs:label "declared for digital object type"@en ;
                                                                   <http://www.w3.org/2004/02/skos/core#definition> "Connects a FIP declaration to the digital object type it applies to"@en .


###  https://w3id.org/fair/fip/terms/declares-current-use-of
<https://w3id.org/fair/fip/terms/declares-current-use-of> rdf:type owl:ObjectProperty ;
                                                          rdfs:domain <https://w3id.org/fair/fip/terms/FAIR-Declaration> ;
                                                          rdfs:range <https://w3id.org/fair/fip/terms/Available-FAIR-Supporting-Resource> ;
                                                          rdfs:isDefinedBy <https://w3id.org/fair/fip/latest/declares-current-use-of> ;
                                                          rdfs:label "declares current use of"@en ;
                                                          <http://www.w3.org/2004/02/skos/core#definition> "Connects a FIP declaration to the resource that the community thereby declares to currently use"@en .


###  https://w3id.org/fair/fip/terms/declares-planned-development-of
<https://w3id.org/fair/fip/terms/declares-planned-development-of> rdf:type owl:ObjectProperty ;
                                                                  rdfs:domain <https://w3id.org/fair/fip/terms/FAIR-Declaration> ;
                                                                  rdfs:range <https://w3id.org/fair/fip/terms/FAIR-Supporting-Resource-to-be-Developed> ;
                                                                  rdfs:isDefinedBy <https://w3id.org/fair/fip/latest/declares-planned-development-of> ;
                                                                  rdfs:label "declares planned development of"@en ;
                                                                  <http://www.w3.org/2004/02/skos/core#definition> "Connects a FIP declaration to the resource that the community thereby declares to plan to develop"@en .


###  https://w3id.org/fair/fip/terms/declares-planned-replacement-of
<https://w3id.org/fair/fip/terms/declares-planned-replacement-of> rdf:type owl:ObjectProperty ;
                                                                  rdfs:domain <https://w3id.org/fair/fip/terms/FAIR-Declaration> ;
                                                                  rdfs:range <https://w3id.org/fair/fip/terms/Available-FAIR-Supporting-Resource> ;
                                                                  rdfs:isDefinedBy <https://w3id.org/fair/fip/latest/declares-planned-replacement-of> ;
                                                                  rdfs:label "declares planned replacement of"@en ;
                                                                  <http://www.w3.org/2004/02/skos/core#definition> "Connects a FIP declaration to the resource that the community thereby declares to plan to replace in the future. The same declaration should also state a resource that the community declares to plan to use instead (with fip:declares-planned-use-of)."@en .


###  https://w3id.org/fair/fip/terms/declares-planned-use-of
<https://w3id.org/fair/fip/terms/declares-planned-use-of> rdf:type owl:ObjectProperty ;
                                                          rdfs:domain <https://w3id.org/fair/fip/terms/FAIR-Declaration> ;
                                                          rdfs:range <https://w3id.org/fair/fip/terms/FAIR-Supporting-Resource> ;
                                                          rdfs:isDefinedBy <https://w3id.org/fair/fip/latest/declares-planned-use-of> ;
                                                          rdfs:label "declares planned use of"@en ;
                                                          <http://www.w3.org/2004/02/skos/core#definition> "Connects a FIP declaration to the resource that the community thereby declares to plan to use in the future"@en .


###  https://w3id.org/fair/fip/terms/has-data-steward
<https://w3id.org/fair/fip/terms/has-data-steward> rdf:type owl:ObjectProperty ;
                                                   rdfs:subPropertyOf <http://xmlns.com/foaf/0.1/member> ;
                                                   rdfs:domain <https://w3id.org/fair/fip/terms/FAIR-Implementation-Community> ;
                                                   rdfs:isDefinedBy <https://w3id.org/fair/fip/latest/has-data-steward> ;
                                                   rdfs:label "has data steward"@en ;
                                                   <http://www.w3.org/2004/02/skos/core#definition> "Specifies the data steward for a FAIR implementation community"@en .


###  https://w3id.org/fair/fip/terms/has-declaration-index
<https://w3id.org/fair/fip/terms/has-declaration-index> rdf:type owl:ObjectProperty ;
                                                        rdfs:domain <https://w3id.org/fair/fip/terms/FAIR-Supporting-Resource> ;
                                                        rdfs:range <http://purl.org/nanopub/x/NanopubIndex> ;
                                                        rdfs:isDefinedBy <https://w3id.org/fair/fip/latest/has-declaration-index> ;
                                                        rdfs:label "has declaration index"@en ;
                                                        <http://www.w3.org/2004/02/skos/core#definition> "Connects a FAIR Implementation Profile or a Semantic Interoperability Profile to the index of their declarations."@en .


###  https://w3id.org/fair/fip/terms/refers-to-principle
<https://w3id.org/fair/fip/terms/refers-to-principle> rdf:type owl:ObjectProperty ;
                                                      rdfs:range <https://w3id.org/fair/principles/terms/FAIR-Principle-or-SubPrinciple> ;
                                                      rdfs:isDefinedBy <https://w3id.org/fair/fip/latest/refers-to-principle> ;
                                                      rdfs:label "refers to principle"@en ;
                                                      <http://www.w3.org/2004/02/skos/core#definition> "Connects an entity (for example a FIP declaration) to a FAIR (sub)principle it refers to"@en .


###  https://w3id.org/fair/fip/terms/refers-to-question
<https://w3id.org/fair/fip/terms/refers-to-question> rdf:type owl:ObjectProperty ;
                                                     rdfs:domain <https://w3id.org/fair/fip/terms/FIP-Declaration> ;
                                                     rdfs:range <https://w3id.org/fair/fip/terms/FIP-Question> ;
                                                     rdfs:isDefinedBy <https://w3id.org/fair/fip/latest/refers-to-question> ;
                                                     rdfs:label "refers to question"@en ;
                                                     <http://www.w3.org/2004/02/skos/core#definition> "Connects a FIP declaration to the FIP question it is addressing"@en .


#################################################################
#    Data properties
#################################################################

###  https://w3id.org/fair/fip/terms/considerations
<https://w3id.org/fair/fip/terms/considerations> rdf:type owl:DatatypeProperty ;
                                                 rdfs:domain <https://w3id.org/fair/fip/terms/FAIR-Declaration> ;
                                                 rdfs:isDefinedBy <https://w3id.org/fair/fip/latest/considerations> ;
                                                 rdfs:label "considerations"@en ;
                                                 <http://www.w3.org/2004/02/skos/core#definition> "Considerations that led to a given FIP declaration"@en .


#################################################################
#    Classes
#################################################################

###  http://purl.org/nanopub/x/NanopubIndex
<http://purl.org/nanopub/x/NanopubIndex> rdf:type owl:Class ;
                                         rdfs:label "Nanopublication Index" .


###  https://w3id.org/fair/fip/terms/Authentication-and-authorization-service
<https://w3id.org/fair/fip/terms/Authentication-and-authorization-service> rdf:type owl:Class ;
                                                                           rdfs:subClassOf <https://w3id.org/fair/fip/terms/FAIR-Enabling-Resource> ,
                                                                                           <https://w3id.org/fair/fip/terms/FAIR-Supporting-Service> ;
                                                                           rdfs:isDefinedBy <https://w3id.org/fair/fip/latest/Authentication-and-authorization-service> ;
                                                                           rdfs:label "Authentication and authorization service"@en ;
                                                                           <http://www.w3.org/2004/02/skos/core#definition> "A service that mediates access to digital objects according to specifed conditions."@en .


###  https://w3id.org/fair/fip/terms/Available-FAIR-Enabling-Resource
<https://w3id.org/fair/fip/terms/Available-FAIR-Enabling-Resource> rdf:type owl:Class ;
                                                                   rdfs:subClassOf <https://w3id.org/fair/fip/terms/Available-FAIR-Supporting-Resource> ,
                                                                                   <https://w3id.org/fair/fip/terms/FAIR-Enabling-Resource> ;
                                                                   rdfs:isDefinedBy <https://w3id.org/fair/fip/latest/Available-FAIR-Enabling-Resource> ;
                                                                   rdfs:label "Available FAIR-Enabling Resource"@en ;
                                                                   <http://www.w3.org/2004/02/skos/core#definition> "A FAIR-enabling resource that is available for use"@en .


###  https://w3id.org/fair/fip/terms/Available-FAIR-Supporting-Resource
<https://w3id.org/fair/fip/terms/Available-FAIR-Supporting-Resource> rdf:type owl:Class ;
                                                                     rdfs:subClassOf <https://w3id.org/fair/fip/terms/FAIR-Supporting-Resource> ;
                                                                     rdfs:isDefinedBy <https://w3id.org/fair/fip/latest/Available-FAIR-Supporting-Resource> ;
                                                                     rdfs:label "Available FAIR Supporting Resource"@en ;
                                                                     <http://www.w3.org/2004/02/skos/core#definition> "A FAIR Supporting Resource that is available for use."@en .


###  https://w3id.org/fair/fip/terms/Communication-protocol
<https://w3id.org/fair/fip/terms/Communication-protocol> rdf:type owl:Class ;
                                                         rdfs:subClassOf <https://w3id.org/fair/fip/terms/FAIR-Enabling-Resource> ,
                                                                         <https://w3id.org/fair/fip/terms/FAIR-Specification> ;
                                                         rdfs:isDefinedBy <https://w3id.org/fair/fip/latest/Communication-protocol> ;
                                                         rdfs:label "Communication protocol"@en ;
                                                         <http://www.w3.org/2004/02/skos/core#definition> "A specification of how messages are structured and exchanged."@en .


###  https://w3id.org/fair/fip/terms/Cross-Domain-Community
<https://w3id.org/fair/fip/terms/Cross-Domain-Community> rdf:type owl:Class ;
                                                         rdfs:subClassOf <https://w3id.org/fair/fip/terms/FAIR-Implementation-Community> ;
                                                         rdfs:isDefinedBy <https://w3id.org/fair/fip/latest/Cross-Domain-Community> ;
                                                         rdfs:label "Cross domain community"@en ;
                                                         <http://www.w3.org/2004/02/skos/core#definition> "A FAIR Implementation Communities with cross-domain coverage"@en .


###  https://w3id.org/fair/fip/terms/Crosswalk
<https://w3id.org/fair/fip/terms/Crosswalk> rdf:type owl:Class ;
                                            rdfs:subClassOf <https://w3id.org/fair/fip/terms/FAIR-Specification> ;
                                            rdfs:isDefinedBy <https://w3id.org/fair/fip/latest/Crosswalk> ;
                                            rdfs:label "Crosswalk"@en ;
                                            <http://www.w3.org/2004/02/skos/core#definition> "A specification consisting of a set of rules that define how (meta)data elements or attributes from one schema can be aligned and mapped to (meta)data elements or attributes in another schema that share the same constraints and thus share the same semantic role."@en .


###  https://w3id.org/fair/fip/terms/Data-Steward-Professional-Profile
<https://w3id.org/fair/fip/terms/Data-Steward-Professional-Profile> rdf:type owl:Class ;
                                                                    rdfs:subClassOf <https://w3id.org/fair/fip/terms/FAIR-Supporting-Resource> ;
                                                                    rdfs:isDefinedBy <https://w3id.org/fair/fip/latest/Data-Steward-Professional-Profile> ;
                                                                    rdfs:label "FAIR data steward professional profile"@en ;
                                                                    <http://www.w3.org/2004/02/skos/core#definition> "A document stating the accumulated training qualifications and FAIR outputs authored by or contributed to, by that person. The profile may be augmented with additional statements regarding professional roles and skills."@en .


###  https://w3id.org/fair/fip/terms/Data-usage-license
<https://w3id.org/fair/fip/terms/Data-usage-license> rdf:type owl:Class ;
                                                     rdfs:subClassOf <https://w3id.org/fair/fip/terms/FAIR-Data-Policy> ,
                                                                     <https://w3id.org/fair/fip/terms/FAIR-Enabling-Resource> ;
                                                     rdfs:isDefinedBy <https://w3id.org/fair/fip/latest/Data-usage-license> ;
                                                     rdfs:label "Data usage license"@en ;
                                                     <http://www.w3.org/2004/02/skos/core#definition> "A data policy that specifies legal restrictions on the reuse of the data."@en .


###  https://w3id.org/fair/fip/terms/Digital-Object-Type
<https://w3id.org/fair/fip/terms/Digital-Object-Type> rdf:type owl:Class ;
                                                      rdfs:isDefinedBy <https://w3id.org/fair/fip/latest/Digital-Object-Type> ;
                                                      rdfs:label "Digital Object Type"@en ;
                                                      <http://www.w3.org/2004/02/skos/core#definition> "A digital object type is a classification of digital objects with respect to their informational functions to specify the nature of the digital object and the operations that can be performed on it."@en .


###  https://w3id.org/fair/fip/terms/Domain-Specific-Community
<https://w3id.org/fair/fip/terms/Domain-Specific-Community> rdf:type owl:Class ;
                                                            rdfs:subClassOf <https://w3id.org/fair/fip/terms/FAIR-Implementation-Community> ;
                                                            rdfs:isDefinedBy <https://w3id.org/fair/fip/latest/Domain-Specific-Community> ;
                                                            rdfs:label "Domain specific community"@en ;
                                                            <http://www.w3.org/2004/02/skos/core#definition> "A FAIR Implementation Communities with domain coverage"@en .


###  https://w3id.org/fair/fip/terms/Editor
<https://w3id.org/fair/fip/terms/Editor> rdf:type owl:Class ;
                                         rdfs:subClassOf <https://w3id.org/fair/fip/terms/FAIR-Supporting-Service> ;
                                         rdfs:isDefinedBy <https://w3id.org/fair/fip/latest/Editor> ;
                                         rdfs:label "Editor"@en ;
                                         <http://www.w3.org/2004/02/skos/core#definition> "A service that provides a user-friendly interface for easy editing of metadata, vocabularies or crosswalks."@en .


###  https://w3id.org/fair/fip/terms/FAIR-Case-Study
<https://w3id.org/fair/fip/terms/FAIR-Case-Study> rdf:type owl:Class ;
                                                  rdfs:subClassOf <https://w3id.org/fair/fip/terms/FAIR-Declaration> ;
                                                  rdfs:isDefinedBy <https://w3id.org/fair/fip/latest/FAIR-Case-Study> ;
                                                  rdfs:label "FAIR case study"@en ;
                                                  <http://www.w3.org/2004/02/skos/core#definition> "A description of a real-life situation where FAIR requirements of digital objects play a central role."@en .


###  https://w3id.org/fair/fip/terms/FAIR-Data-Policy
<https://w3id.org/fair/fip/terms/FAIR-Data-Policy> rdf:type owl:Class ;
                                                   rdfs:subClassOf <https://w3id.org/fair/fip/terms/FAIR-Supporting-Resource> ;
                                                   rdfs:isDefinedBy <https://w3id.org/fair/fip/latest/FAIR-Data-Policy> ;
                                                   rdfs:label "FAIR Data Policy"@en ;
                                                   <http://www.w3.org/2004/02/skos/core#definition> "A policy that specifies and guides FAIR data practices for a community."@en .


###  https://w3id.org/fair/fip/terms/FAIR-Data-Stewardship-Event
<https://w3id.org/fair/fip/terms/FAIR-Data-Stewardship-Event> rdf:type owl:Class ;
                                                              rdfs:subClassOf <https://w3id.org/fair/fip/terms/FAIR-Supporting-Resource> ;
                                                              rdfs:isDefinedBy <https://w3id.org/fair/fip/latest/FAIR-Data-Stewardship-Event> ;
                                                              rdfs:label "FAIR data stewardship event"@en ;
                                                              <http://www.w3.org/2004/02/skos/core#definition> "A meeting specifically designed for current or aspiring data stewards to provide a rigorous understanding of the FAIR principles from theory to their concrete implementation."@en .


###  https://w3id.org/fair/fip/terms/FAIR-Data-Stewardship-Plan-Template
<https://w3id.org/fair/fip/terms/FAIR-Data-Stewardship-Plan-Template> rdf:type owl:Class ;
                                                                      rdfs:subClassOf <https://w3id.org/fair/fip/terms/FAIR-Supporting-Resource> ;
                                                                      rdfs:isDefinedBy <https://w3id.org/fair/fip/latest/FAIR-Data-Stewardship-Plan-Template> ;
                                                                      rdfs:label "FAIR data stewardship plan template"@en ;
                                                                      <http://www.w3.org/2004/02/skos/core#definition> "A template guiding data stewardship including how FAIR Principles should be implemented. The template must be completed with project-specific information in any given instance to outline how data are to be handled in preparation for the project,  during the research project, and after the project is completed."@en .


###  https://w3id.org/fair/fip/terms/FAIR-Declaration
<https://w3id.org/fair/fip/terms/FAIR-Declaration> rdf:type owl:Class ;
                                                   rdfs:subClassOf <https://w3id.org/fair/fip/terms/FAIR-Supporting-Resource> ;
                                                   rdfs:isDefinedBy <https://w3id.org/fair/fip/latest/FAIR-Declaration> ;
                                                   rdfs:label "FAIR Declaration"@en ;
                                                   <http://www.w3.org/2004/02/skos/core#definition> "The statement of a community on how it addresses a FAIR-related question."@en .


###  https://w3id.org/fair/fip/terms/FAIR-Enabling-Resource
<https://w3id.org/fair/fip/terms/FAIR-Enabling-Resource> rdf:type owl:Class ;
                                                         rdfs:subClassOf <https://w3id.org/fair/fip/terms/FAIR-Supporting-Resource> ;
                                                         rdfs:isDefinedBy <https://w3id.org/fair/fip/latest/FAIR-Enabling-Resource> ;
                                                         rdfs:label "FAIR-Enabling Resource"@en ;
                                                         <http://www.w3.org/2004/02/skos/core#definition> "A service, a specification or a data policy that is essential to the operationalization of the FAIR Principles, i.e., puts FAIR into action. A FAIR-Enabling Resource (FER) provides a function needed to achieve some aspect of FAIR behavior and is explicitly linked to one or more FAIR principles."@en .


###  https://w3id.org/fair/fip/terms/FAIR-Enabling-Resource-to-be-Developed
<https://w3id.org/fair/fip/terms/FAIR-Enabling-Resource-to-be-Developed> rdf:type owl:Class ;
                                                                         rdfs:subClassOf <https://w3id.org/fair/fip/terms/FAIR-Enabling-Resource> ,
                                                                                         <https://w3id.org/fair/fip/terms/FAIR-Supporting-Resource-to-be-Developed> ;
                                                                         rdfs:isDefinedBy <https://w3id.org/fair/fip/latest/FAIR-Enabling-Resource-to-be-Developed> ;
                                                                         rdfs:label "FAIR-Enabling Resource to be Developed"@en ;
                                                                         <http://www.w3.org/2004/02/skos/core#definition> "A FAIR-enabling resource that is not yet available but still needs to be developed"@en .


###  https://w3id.org/fair/fip/terms/FAIR-Implementation-Community
<https://w3id.org/fair/fip/terms/FAIR-Implementation-Community> rdf:type owl:Class ;
                                                                rdfs:subClassOf <https://w3id.org/fair/fip/terms/FAIR-Supporting-Resource> ;
                                                                rdfs:isDefinedBy <https://w3id.org/fair/fip/latest/FAIR-Implementation-Community> ;
                                                                rdfs:label "FAIR Implementation Community"@en ;
                                                                <http://www.w3.org/2004/02/skos/core#definition> "A FAIR Implementation Community (FIC) is a self-identified collection of people and/or organizations with the aim to implement the FAIR Principles"@en .


###  https://w3id.org/fair/fip/terms/FAIR-Implementation-Profile
<https://w3id.org/fair/fip/terms/FAIR-Implementation-Profile> rdf:type owl:Class ;
                                                              rdfs:subClassOf <https://w3id.org/fair/fip/terms/FAIR-Enabling-Resource> ;
                                                              rdfs:isDefinedBy <https://w3id.org/fair/fip/latest/FAIR-Implementation-Profile> ;
                                                              rdfs:label "FAIR Implementation Profile"@en ;
                                                              <http://www.w3.org/2004/02/skos/core#definition> "A FAIR Implementation Profile (FIP) is a list of declared technology choices intended to implement each of the FAIR Guiding Principles, made as a collective decision by the members of a particular community of practice. "@en .


###  https://w3id.org/fair/fip/terms/FAIR-Interpretation
<https://w3id.org/fair/fip/terms/FAIR-Interpretation> rdf:type owl:Class ;
                                                      rdfs:subClassOf <https://w3id.org/fair/fip/terms/FAIR-Declaration> ;
                                                      rdfs:isDefinedBy <https://w3id.org/fair/fip/latest/FAIR-Interpretation> ;
                                                      rdfs:label "FAIR interpretation"@en ;
                                                      <http://www.w3.org/2004/02/skos/core#definition> "A theoretical and practical explanation of the FAIR Principle by a recognized expert authority."@en .


###  https://w3id.org/fair/fip/terms/FAIR-Practice
<https://w3id.org/fair/fip/terms/FAIR-Practice> rdf:type owl:Class ;
                                                rdfs:subClassOf <https://w3id.org/fair/fip/terms/FAIR-Supporting-Resource> ;
                                                rdfs:isDefinedBy <https://w3id.org/fair/fip/latest/FAIR-Practice> ;
                                                rdfs:label "FAIR practice"@en ;
                                                <http://www.w3.org/2004/02/skos/core#definition> "A method description detailing the use of a specific resource or a combination of resources as applied by a community to achieve FAIR processing of information."@en .


###  https://w3id.org/fair/fip/terms/FAIR-Qualification-Criteria
<https://w3id.org/fair/fip/terms/FAIR-Qualification-Criteria> rdf:type owl:Class ;
                                                              rdfs:subClassOf <https://w3id.org/fair/fip/terms/FAIR-Declaration> ;
                                                              rdfs:isDefinedBy <https://w3id.org/fair/fip/latest/FAIR-Qualification-Criteria> ;
                                                              rdfs:label "FAIR Qualifcation Criteria"@en ;
                                                              <http://www.w3.org/2004/02/skos/core#definition> "A proposition on which a qualification of FAIR Supporting Resources is based."@en .


###  https://w3id.org/fair/fip/terms/FAIR-Representation-Service
<https://w3id.org/fair/fip/terms/FAIR-Representation-Service> rdf:type owl:Class ;
                                                              rdfs:subClassOf <https://w3id.org/fair/fip/terms/FAIR-Supporting-Service> ;
                                                              rdfs:isDefinedBy <https://w3id.org/fair/fip/latest/FAIR-Representation-Service> ;
                                                              rdfs:label "FAIR Representation Service"@en ;
                                                              <http://www.w3.org/2004/02/skos/core#definition> "A transformation service that converts non-FAIR data into a FAIR representation using machine-readable knowledge representation languages."@en .


###  https://w3id.org/fair/fip/terms/FAIR-Specification
<https://w3id.org/fair/fip/terms/FAIR-Specification> rdf:type owl:Class ;
                                                     rdfs:subClassOf <https://w3id.org/fair/fip/terms/FAIR-Supporting-Resource> ;
                                                     rdfs:isDefinedBy <https://w3id.org/fair/fip/latest/FAIR-Specification> ;
                                                     rdfs:label "FAIR specification"@en ;
                                                     <http://www.w3.org/2004/02/skos/core#definition> "A precise description of features, requirements, constraints and recommendations for a specific implementation of a component, system or service supporting the implementation of the FAIR principles."@en .


###  https://w3id.org/fair/fip/terms/FAIR-Supporting-Resource
<https://w3id.org/fair/fip/terms/FAIR-Supporting-Resource> rdf:type owl:Class ;
                                                           rdfs:isDefinedBy <https://w3id.org/fair/fip/latest/FAIR-Supporting-Resource> ;
                                                           rdfs:label "FAIR Supporting Resource"@en ;
                                                           <http://www.w3.org/2004/02/skos/core#definition> "Any resource that supports FAIR Data Stewardship. FSRs are represented as FAIR Digital Objects (using the nanopublication framework) with Globally Unique, Persistent, Resolvable Identifiers (GUPRI) that resolve to machine-readable metadata about the resource."@en .


###  https://w3id.org/fair/fip/terms/FAIR-Supporting-Resource-to-be-Developed
<https://w3id.org/fair/fip/terms/FAIR-Supporting-Resource-to-be-Developed> rdf:type owl:Class ;
                                                                           rdfs:subClassOf <https://w3id.org/fair/fip/terms/FAIR-Supporting-Resource> ;
                                                                           rdfs:isDefinedBy <https://w3id.org/fair/fip/latest/FAIR-Supporting-Resource-to-be-Developed> ;
                                                                           rdfs:label "FAIR Supporting Resource to be developed"@en ;
                                                                           <http://www.w3.org/2004/02/skos/core#definition> "A FAIR Supporting Resource that is not yet available but still needs to be developed."@en .


###  https://w3id.org/fair/fip/terms/FAIR-Supporting-Service
<https://w3id.org/fair/fip/terms/FAIR-Supporting-Service> rdf:type owl:Class ;
                                                          rdfs:subClassOf <https://w3id.org/fair/fip/terms/FAIR-Supporting-Resource> ;
                                                          rdfs:isDefinedBy <https://w3id.org/fair/fip/latest/FAIR-Supporting-Service> ;
                                                          rdfs:label "FAIR supporting service"@en ;
                                                          <http://www.w3.org/2004/02/skos/core#definition> "Any online accessible software system or component that supports the implementation of the FAIR Principles."@en .


###  https://w3id.org/fair/fip/terms/FAIR-Training-Material
<https://w3id.org/fair/fip/terms/FAIR-Training-Material> rdf:type owl:Class ;
                                                         rdfs:subClassOf <https://w3id.org/fair/fip/terms/FAIR-Supporting-Resource> ;
                                                         rdfs:isDefinedBy <https://w3id.org/fair/fip/latest/FAIR-Training-Material> ;
                                                         rdfs:label "FAIR training material"@en ;
                                                         <http://www.w3.org/2004/02/skos/core#definition> "Any educational resource (such as the content or its published representation in text, presentation graphics, or video) that covers FAIR topics of interest."@en .


###  https://w3id.org/fair/fip/terms/FIP-Data-related-Question
<https://w3id.org/fair/fip/terms/FIP-Data-related-Question> rdf:type owl:Class ;
                                                            rdfs:subClassOf <https://w3id.org/fair/fip/terms/FIP-Question> ;
                                                            rdfs:isDefinedBy <https://w3id.org/fair/fip/latest/FIP-Data-related-Question> ;
                                                            rdfs:label "FIP Data-related Question"@en ;
                                                            <http://www.w3.org/2004/02/skos/core#definition> "A FIP question that is relevant for the actual data (as compared to just their metadata)"@en .


###  https://w3id.org/fair/fip/terms/FIP-Declaration
<https://w3id.org/fair/fip/terms/FIP-Declaration> rdf:type owl:Class ;
                                                  rdfs:subClassOf <https://w3id.org/fair/fip/terms/FAIR-Declaration> ;
                                                  rdfs:isDefinedBy <https://w3id.org/fair/fip/latest/FIP-Declaration> ;
                                                  rdfs:label "FIP Declaration"@en ;
                                                  <http://www.w3.org/2004/02/skos/core#definition> "The expression of a community on how they address a FIP question"@en .


###  https://w3id.org/fair/fip/terms/FIP-Metadata-related-Question
<https://w3id.org/fair/fip/terms/FIP-Metadata-related-Question> rdf:type owl:Class ;
                                                                rdfs:subClassOf <https://w3id.org/fair/fip/terms/FIP-Question> ;
                                                                rdfs:isDefinedBy <https://w3id.org/fair/fip/latest/FIP-Metadata-related-Question> ;
                                                                rdfs:label "FIP Metadata-related Question"@en ;
                                                                <http://www.w3.org/2004/02/skos/core#definition> "A FIP question that is relevant for metadata (as compared to the data themselves)"@en .


###  https://w3id.org/fair/fip/terms/FIP-No-Choice-Declaration
<https://w3id.org/fair/fip/terms/FIP-No-Choice-Declaration> rdf:type owl:Class ;
                                                            rdfs:subClassOf <https://w3id.org/fair/fip/terms/FIP-Declaration> ;
                                                            rdfs:isDefinedBy <https://w3id.org/fair/fip/latest/FIP-No-Choice-Declaration> ;
                                                            rdfs:label "FIP No-Choice Declaration"@en ;
                                                            <http://www.w3.org/2004/02/skos/core#definition> "A declaration stating that no choice has been made (yet)"@en .


###  https://w3id.org/fair/fip/terms/FIP-Question
<https://w3id.org/fair/fip/terms/FIP-Question> rdf:type owl:Class ;
                                               rdfs:isDefinedBy <https://w3id.org/fair/fip/latest/FIP-Question> ;
                                               rdfs:label "FIP Question"@en ;
                                               <http://www.w3.org/2004/02/skos/core#definition> "A question communities have to address when declaring their FAIR Implementation Profiles"@en .


###  https://w3id.org/fair/fip/terms/FSR-Declaration
<https://w3id.org/fair/fip/terms/FSR-Declaration> rdf:type owl:Class ;
                                                  rdfs:subClassOf <https://w3id.org/fair/fip/terms/FAIR-Declaration> ;
                                                  rdfs:isDefinedBy <https://w3id.org/fair/fip/latest/FSR-Declaration> ;
                                                  rdfs:label "FSR Declaration"@en ;
                                                  <http://www.w3.org/2004/02/skos/core#definition> "The statement of a community on the usage of a FAIR Supporting Resource."@en .


###  https://w3id.org/fair/fip/terms/Identifier-service
<https://w3id.org/fair/fip/terms/Identifier-service> rdf:type owl:Class ;
                                                     rdfs:subClassOf <https://w3id.org/fair/fip/terms/FAIR-Enabling-Resource> ,
                                                                     <https://w3id.org/fair/fip/terms/FAIR-Supporting-Service> ;
                                                     rdfs:isDefinedBy <https://w3id.org/fair/fip/latest/Identifier-service> ;
                                                     rdfs:label "Identifier service"@en ;
                                                     <http://www.w3.org/2004/02/skos/core#definition> "A service that provides for any digital object (1) algorithms guaranteeing global uniqueness, (2) policy document that guarantees persistent and (3) resolution of the identifier to machine-actionable metadata describing the object and its location."@en .


###  https://w3id.org/fair/fip/terms/Knowledge-representation-language
<https://w3id.org/fair/fip/terms/Knowledge-representation-language> rdf:type owl:Class ;
                                                                    rdfs:subClassOf <https://w3id.org/fair/fip/terms/FAIR-Enabling-Resource> ,
                                                                                    <https://w3id.org/fair/fip/terms/FAIR-Specification> ;
                                                                    rdfs:isDefinedBy <https://w3id.org/fair/fip/latest/Knowledge-representation-language> ;
                                                                    rdfs:label "Knowledge representation language"@en ;
                                                                    <http://www.w3.org/2004/02/skos/core#definition> "A language specification that enables knowledge to be processed by machines."@en .


###  https://w3id.org/fair/fip/terms/Metadata-data-linking-schema
<https://w3id.org/fair/fip/terms/Metadata-data-linking-schema> rdf:type owl:Class ;
                                                               rdfs:subClassOf <https://w3id.org/fair/fip/terms/FAIR-Enabling-Resource> ,
                                                                               <https://w3id.org/fair/fip/terms/FAIR-Specification> ;
                                                               rdfs:isDefinedBy <https://w3id.org/fair/fip/latest/Metadata-data-linking-schema> ;
                                                               rdfs:label "Metadata-data linking schema"@en ;
                                                               <http://www.w3.org/2004/02/skos/core#definition> "A specification that provides a unique, persistent, (ideally) bi-directional, machine-actionable link between metadata and the data they describe."@en .


###  https://w3id.org/fair/fip/terms/Metadata-preservation-policy
<https://w3id.org/fair/fip/terms/Metadata-preservation-policy> rdf:type owl:Class ;
                                                               rdfs:subClassOf <https://w3id.org/fair/fip/terms/FAIR-Data-Policy> ,
                                                                               <https://w3id.org/fair/fip/terms/FAIR-Enabling-Resource> ;
                                                               rdfs:isDefinedBy <https://w3id.org/fair/fip/latest/Metadata-preservation-policy> ;
                                                               rdfs:label "Metadata preservation policy"@en ;
                                                               <http://www.w3.org/2004/02/skos/core#definition> "A data policy that describes the conditions under which metadata should be provided in the future."@en .


###  https://w3id.org/fair/fip/terms/Metadata-schema
<https://w3id.org/fair/fip/terms/Metadata-schema> rdf:type owl:Class ;
                                                  rdfs:subClassOf <https://w3id.org/fair/fip/terms/FAIR-Enabling-Resource> ,
                                                                  <https://w3id.org/fair/fip/terms/FAIR-Specification> ;
                                                  rdfs:isDefinedBy <https://w3id.org/fair/fip/latest/Metadata-schema> ;
                                                  rdfs:label "Metadata schema"@en ;
                                                  <http://www.w3.org/2004/02/skos/core#definition> "A specification that specifies the structured representation of metadata describing attributes of data or other digital objects in terms of semantics, syntax and optionality."@en .


###  https://w3id.org/fair/fip/terms/Provenance-Tracking-Service
<https://w3id.org/fair/fip/terms/Provenance-Tracking-Service> rdf:type owl:Class ;
                                                              rdfs:subClassOf <https://w3id.org/fair/fip/terms/FAIR-Supporting-Service> ;
                                                              rdfs:isDefinedBy <https://w3id.org/fair/fip/latest/Provenance-Tracking-Service> ;
                                                              rdfs:label "Provenance tracking service"@en ;
                                                              <http://www.w3.org/2004/02/skos/core#definition> "A system that systematically captures, stores and manages detailed information about the origin, history, and lifecycle of digital objects creating metadata based on a provenance model. "@en .


###  https://w3id.org/fair/fip/terms/Provenance-model
<https://w3id.org/fair/fip/terms/Provenance-model> rdf:type owl:Class ;
                                                   rdfs:subClassOf <https://w3id.org/fair/fip/terms/FAIR-Enabling-Resource> ,
                                                                   <https://w3id.org/fair/fip/terms/FAIR-Specification> ;
                                                   rdfs:isDefinedBy <https://w3id.org/fair/fip/latest/Provenance-model> ;
                                                   rdfs:label "Provenance model"@en ;
                                                   <http://www.w3.org/2004/02/skos/core#definition> "A specification that specifies metadata describing the origin and lineage of data or other digital objects."@en .


###  https://w3id.org/fair/fip/terms/Registry
<https://w3id.org/fair/fip/terms/Registry> rdf:type owl:Class ;
                                           rdfs:subClassOf <https://w3id.org/fair/fip/terms/FAIR-Enabling-Resource> ,
                                                           <https://w3id.org/fair/fip/terms/FAIR-Supporting-Service> ;
                                           rdfs:isDefinedBy <https://w3id.org/fair/fip/latest/Registry> ;
                                           rdfs:label "Registry"@en ;
                                           <http://www.w3.org/2004/02/skos/core#definition> "A service that indexes metadata and data and provides search over that index."@en .


###  https://w3id.org/fair/fip/terms/SIP-Declaration
<https://w3id.org/fair/fip/terms/SIP-Declaration> rdf:type owl:Class ;
                                                  rdfs:subClassOf <https://w3id.org/fair/fip/terms/FAIR-Declaration> ;
                                                  rdfs:isDefinedBy <https://w3id.org/fair/fip/latest/SIP-Declaration> ;
                                                  rdfs:label "SIP Declaration"@en ;
                                                  <http://www.w3.org/2004/02/skos/core#definition> "The statement of a community on how it addresses a SIP question."@en .


###  https://w3id.org/fair/fip/terms/Semantic-Interoperability-Profile
<https://w3id.org/fair/fip/terms/Semantic-Interoperability-Profile> rdf:type owl:Class ;
                                                                    rdfs:subClassOf <https://w3id.org/fair/fip/terms/FAIR-Supporting-Resource> ;
                                                                    rdfs:isDefinedBy <https://w3id.org/fair/fip/latest/Semantic-Interoperability-Profile> ;
                                                                    rdfs:label "Semantic Interoperability Profile"@en ;
                                                                    <http://www.w3.org/2004/02/skos/core#definition> "A Semantic Interoperability Profil (SIP) is a list of FAIR Supporting Resources chosen by a community to support semantic interoperability of (meta)data."@en .


###  https://w3id.org/fair/fip/terms/Semantic-model
<https://w3id.org/fair/fip/terms/Semantic-model> rdf:type owl:Class ;
                                                 rdfs:subClassOf <https://w3id.org/fair/fip/terms/FAIR-Enabling-Resource> ,
                                                                 <https://w3id.org/fair/fip/terms/FAIR-Specification> ;
                                                 rdfs:isDefinedBy <https://w3id.org/fair/fip/latest/Semantic-model> ;
                                                 rdfs:label "Semantic model"@en ;
                                                 <http://www.w3.org/2004/02/skos/core#definition> "A specification that defines qualified relations between entities describing data or other digital objects according to the Linked Data principles. This can include semantic data models and ontologies."@en .


###  https://w3id.org/fair/fip/terms/Specific-Community
<https://w3id.org/fair/fip/terms/Specific-Community> rdf:type owl:Class ;
                                                     rdfs:subClassOf <https://w3id.org/fair/fip/terms/FAIR-Implementation-Community> ;
                                                     rdfs:isDefinedBy <https://w3id.org/fair/fip/latest/Specific-Community> ;
                                                     rdfs:label "Specific community"@en ;
                                                     <http://www.w3.org/2004/02/skos/core#definition> "A FAIR Implementation Communities with specific coverage within a domain"@en .


###  https://w3id.org/fair/fip/terms/Structured-vocabulary
<https://w3id.org/fair/fip/terms/Structured-vocabulary> rdf:type owl:Class ;
                                                        rdfs:subClassOf <https://w3id.org/fair/fip/terms/FAIR-Enabling-Resource> ,
                                                                        <https://w3id.org/fair/fip/terms/FAIR-Specification> ;
                                                        rdfs:isDefinedBy <https://w3id.org/fair/fip/latest/Structured-vocabulary> ;
                                                        rdfs:label "Structured vocabulary"@en ;
                                                        <http://www.w3.org/2004/02/skos/core#definition> "A specification for a controlled list of uniquely identified and unambigous concepts with their definitions represented using web standards."@en .


###  https://w3id.org/fair/fip/terms/Validation-Service
<https://w3id.org/fair/fip/terms/Validation-Service> rdf:type owl:Class ;
                                                     rdfs:subClassOf <https://w3id.org/fair/fip/terms/FAIR-Supporting-Service> ;
                                                     rdfs:isDefinedBy <https://w3id.org/fair/fip/latest/Validation-Service> ;
                                                     rdfs:label "Validation service"@en ;
                                                     <http://www.w3.org/2004/02/skos/core#definition> "A system that automatically verifies the accuracy, completeness, or compliance of data, code or processes against predefined criteria or standards."@en .


###  https://w3id.org/fair/fip/terms/Web-API
<https://w3id.org/fair/fip/terms/Web-API> rdf:type owl:Class ;
                                          rdfs:subClassOf <https://w3id.org/fair/fip/terms/FAIR-Supporting-Service> ;
                                          rdfs:isDefinedBy <https://w3id.org/fair/fip/latest/Web-API> ;
                                          rdfs:label "Web-API"@en ;
                                          <http://www.w3.org/2004/02/skos/core#definition> "An Application Programming Interface (API) for the World Wide Web that allows different software applications to communicate with each other."@en .


###  https://w3id.org/fair/principles/terms/FAIR-Principle-or-SubPrinciple
<https://w3id.org/fair/principles/terms/FAIR-Principle-or-SubPrinciple> rdf:type owl:Class ;
                                                                        rdfs:label "FAIR Principle or Sub-Principle" .


#################################################################
#    Individuals
#################################################################

###  https://w3id.org/fair/fip/terms/FIP-Question-A1.1-D
<https://w3id.org/fair/fip/terms/FIP-Question-A1.1-D> rdf:type owl:NamedIndividual ,
                                                               <https://w3id.org/fair/fip/terms/FIP-Question> ;
                                                      <https://w3id.org/fair/fip/terms/refers-to-principle> <https://w3id.org/fair/principles/terms/A1.1> ;
                                                      rdfs:isDefinedBy <https://w3id.org/fair/fip/latest/FIP-Question-A1.1-D> ;
                                                      rdfs:label "FIP Question A1.1-D"@en ;
                                                      <http://www.w3.org/2004/02/skos/core#definition> "Which standardized communication protocol do you use for datasets?"@en .


###  https://w3id.org/fair/fip/terms/FIP-Question-A1.1-MD
<https://w3id.org/fair/fip/terms/FIP-Question-A1.1-MD> rdf:type owl:NamedIndividual ,
                                                                <https://w3id.org/fair/fip/terms/FIP-Question> ;
                                                       <https://w3id.org/fair/fip/terms/refers-to-principle> <https://w3id.org/fair/principles/terms/A1.1> ;
                                                       rdfs:isDefinedBy <https://w3id.org/fair/fip/latest/FIP-Question-A1.1-MD> ;
                                                       rdfs:label "FIP Question A1.1-MD"@en ;
                                                       <http://www.w3.org/2004/02/skos/core#definition> "Which standardized communication protocol do you use for metadata records?"@en .


###  https://w3id.org/fair/fip/terms/FIP-Question-A1.2-D
<https://w3id.org/fair/fip/terms/FIP-Question-A1.2-D> rdf:type owl:NamedIndividual ,
                                                               <https://w3id.org/fair/fip/terms/FIP-Question> ;
                                                      <https://w3id.org/fair/fip/terms/refers-to-principle> <https://w3id.org/fair/principles/terms/A1.2> ;
                                                      rdfs:isDefinedBy <https://w3id.org/fair/fip/latest/FIP-Question-A1.2-D> ;
                                                      rdfs:label "FIP Question A1.2-D"@en ;
                                                      <http://www.w3.org/2004/02/skos/core#definition> "Which authentication & authorisation technique do you use for datasets?"@en .


###  https://w3id.org/fair/fip/terms/FIP-Question-A1.2-MD
<https://w3id.org/fair/fip/terms/FIP-Question-A1.2-MD> rdf:type owl:NamedIndividual ,
                                                                <https://w3id.org/fair/fip/terms/FIP-Question> ;
                                                       <https://w3id.org/fair/fip/terms/refers-to-principle> <https://w3id.org/fair/principles/terms/A1.2> ;
                                                       rdfs:isDefinedBy <https://w3id.org/fair/fip/latest/FIP-Question-A1.2-MD> ;
                                                       rdfs:label "FIP Question A1.2-MD"@en ;
                                                       <http://www.w3.org/2004/02/skos/core#definition> "Which authentication & authorisation technique do you use for metadata records?"@en .


###  https://w3id.org/fair/fip/terms/FIP-Question-A2
<https://w3id.org/fair/fip/terms/FIP-Question-A2> rdf:type owl:NamedIndividual ,
                                                           <https://w3id.org/fair/fip/terms/FIP-Question> ;
                                                  <https://w3id.org/fair/fip/terms/refers-to-principle> <https://w3id.org/fair/principles/terms/A2> ;
                                                  rdfs:isDefinedBy <https://w3id.org/fair/fip/latest/FIP-Question-A2> ;
                                                  rdfs:label "FIP Question A2"@en ;
                                                  <http://www.w3.org/2004/02/skos/core#definition> "Which metadata longevity plan do you use?"@en .


###  https://w3id.org/fair/fip/terms/FIP-Question-F1-D
<https://w3id.org/fair/fip/terms/FIP-Question-F1-D> rdf:type owl:NamedIndividual ,
                                                             <https://w3id.org/fair/fip/terms/FIP-Question> ;
                                                    <https://w3id.org/fair/fip/terms/refers-to-principle> <https://w3id.org/fair/principles/terms/F1> ;
                                                    rdfs:isDefinedBy <https://w3id.org/fair/fip/latest/FIP-Question-F1-D> ;
                                                    rdfs:label "FIP Question F1-D"@en ;
                                                    <http://www.w3.org/2004/02/skos/core#definition> "What globally unique, persistent, resolvable identifiers do you use for datasets?"@en .


###  https://w3id.org/fair/fip/terms/FIP-Question-F1-MD
<https://w3id.org/fair/fip/terms/FIP-Question-F1-MD> rdf:type owl:NamedIndividual ,
                                                              <https://w3id.org/fair/fip/terms/FIP-Question> ;
                                                     <https://w3id.org/fair/fip/terms/refers-to-principle> <https://w3id.org/fair/principles/terms/F1> ;
                                                     rdfs:isDefinedBy <https://w3id.org/fair/fip/latest/FIP-Question-F1-MD> ;
                                                     rdfs:label "FIP Question F1-MD"@en ;
                                                     <http://www.w3.org/2004/02/skos/core#definition> "What globally unique, persistent, resolvable identifiers do you use for metadata records?"@en .


###  https://w3id.org/fair/fip/terms/FIP-Question-F2
<https://w3id.org/fair/fip/terms/FIP-Question-F2> rdf:type owl:NamedIndividual ,
                                                           <https://w3id.org/fair/fip/terms/FIP-Question> ;
                                                  <https://w3id.org/fair/fip/terms/refers-to-principle> <https://w3id.org/fair/principles/terms/F2> ;
                                                  rdfs:isDefinedBy <https://w3id.org/fair/fip/latest/FIP-Question-F2> ;
                                                  rdfs:label "FIP Question F2"@en ;
                                                  <http://www.w3.org/2004/02/skos/core#definition> "Which metadata schemas do you use for findability?"@en .


###  https://w3id.org/fair/fip/terms/FIP-Question-F3
<https://w3id.org/fair/fip/terms/FIP-Question-F3> rdf:type owl:NamedIndividual ,
                                                           <https://w3id.org/fair/fip/terms/FIP-Question> ;
                                                  <https://w3id.org/fair/fip/terms/refers-to-principle> <https://w3id.org/fair/principles/terms/F3> ;
                                                  rdfs:isDefinedBy <https://w3id.org/fair/fip/latest/FIP-Question-F3> ;
                                                  rdfs:label "FIP Question F3"@en ;
                                                  <http://www.w3.org/2004/02/skos/core#definition> "What is the technology that links the persistent identifiers of your data to the metadata description?"@en .


###  https://w3id.org/fair/fip/terms/FIP-Question-F4-D
<https://w3id.org/fair/fip/terms/FIP-Question-F4-D> rdf:type owl:NamedIndividual ,
                                                             <https://w3id.org/fair/fip/terms/FIP-Question> ;
                                                    <https://w3id.org/fair/fip/terms/refers-to-principle> <https://w3id.org/fair/principles/terms/F4> ;
                                                    rdfs:isDefinedBy <https://w3id.org/fair/fip/latest/FIP-Question-F4-D> ;
                                                    rdfs:label "FIP Question F4-D"@en ;
                                                    <http://www.w3.org/2004/02/skos/core#definition> "In which search engines are your datasets indexed?"@en .


###  https://w3id.org/fair/fip/terms/FIP-Question-F4-MD
<https://w3id.org/fair/fip/terms/FIP-Question-F4-MD> rdf:type owl:NamedIndividual ,
                                                              <https://w3id.org/fair/fip/terms/FIP-Question> ;
                                                     <https://w3id.org/fair/fip/terms/refers-to-principle> <https://w3id.org/fair/principles/terms/F4> ;
                                                     rdfs:isDefinedBy <https://w3id.org/fair/fip/latest/FIP-Question-F4-MD> ;
                                                     rdfs:label "FIP Question F4-MD"@en ;
                                                     <http://www.w3.org/2004/02/skos/core#definition> "In which search engines are your metadata records indexed?"@en .


###  https://w3id.org/fair/fip/terms/FIP-Question-I1-D
<https://w3id.org/fair/fip/terms/FIP-Question-I1-D> rdf:type owl:NamedIndividual ,
                                                             <https://w3id.org/fair/fip/terms/FIP-Question> ;
                                                    <https://w3id.org/fair/fip/terms/refers-to-principle> <https://w3id.org/fair/principles/terms/I1> ;
                                                    rdfs:isDefinedBy <https://w3id.org/fair/fip/latest/FIP-Question-I1-D> ;
                                                    rdfs:label "FIP Question I1-D"@en ;
                                                    <http://www.w3.org/2004/02/skos/core#definition> "Which knowledge representation languages (allowing machine interoperation) do you use for datasets?"@en .


###  https://w3id.org/fair/fip/terms/FIP-Question-I1-MD
<https://w3id.org/fair/fip/terms/FIP-Question-I1-MD> rdf:type owl:NamedIndividual ,
                                                              <https://w3id.org/fair/fip/terms/FIP-Question> ;
                                                     <https://w3id.org/fair/fip/terms/refers-to-principle> <https://w3id.org/fair/principles/terms/I1> ;
                                                     rdfs:isDefinedBy <https://w3id.org/fair/fip/latest/FIP-Question-I1-MD> ;
                                                     rdfs:label "FIP Question I1-MD"@en ;
                                                     <http://www.w3.org/2004/02/skos/core#definition> "Which knowledge representation languages (allowing machine interoperation) do you use for metadata records?"@en .


###  https://w3id.org/fair/fip/terms/FIP-Question-I2-D
<https://w3id.org/fair/fip/terms/FIP-Question-I2-D> rdf:type owl:NamedIndividual ,
                                                             <https://w3id.org/fair/fip/terms/FIP-Question> ;
                                                    <https://w3id.org/fair/fip/terms/refers-to-principle> <https://w3id.org/fair/principles/terms/I2> ;
                                                    rdfs:isDefinedBy <https://w3id.org/fair/fip/latest/FIP-Question-I2-D> ;
                                                    rdfs:label "FIP Question I2-D"@en ;
                                                    <http://www.w3.org/2004/02/skos/core#definition> "Which structured vocabularies do you use to encode your datasets?"@en .


###  https://w3id.org/fair/fip/terms/FIP-Question-I2-MD
<https://w3id.org/fair/fip/terms/FIP-Question-I2-MD> rdf:type owl:NamedIndividual ,
                                                              <https://w3id.org/fair/fip/terms/FIP-Question> ;
                                                     <https://w3id.org/fair/fip/terms/refers-to-principle> <https://w3id.org/fair/principles/terms/I2> ;
                                                     rdfs:isDefinedBy <https://w3id.org/fair/fip/latest/FIP-Question-I2-MD> ;
                                                     rdfs:label "FIP Question I2-MD"@en ;
                                                     <http://www.w3.org/2004/02/skos/core#definition> "Which structured vocabularies do you use to annotate your metadata records?"@en .


###  https://w3id.org/fair/fip/terms/FIP-Question-I3-D
<https://w3id.org/fair/fip/terms/FIP-Question-I3-D> rdf:type owl:NamedIndividual ,
                                                             <https://w3id.org/fair/fip/terms/FIP-Question> ;
                                                    <https://w3id.org/fair/fip/terms/refers-to-principle> <https://w3id.org/fair/principles/terms/I3> ;
                                                    rdfs:isDefinedBy <https://w3id.org/fair/fip/latest/FIP-Question-I3-D> ;
                                                    rdfs:label "FIP Question I3-D"@en ;
                                                    <http://www.w3.org/2004/02/skos/core#definition> "Which models, schema(s) do you use for your datasets?"@en .


###  https://w3id.org/fair/fip/terms/FIP-Question-I3-MD
<https://w3id.org/fair/fip/terms/FIP-Question-I3-MD> rdf:type owl:NamedIndividual ,
                                                              <https://w3id.org/fair/fip/terms/FIP-Question> ;
                                                     <https://w3id.org/fair/fip/terms/refers-to-principle> <https://w3id.org/fair/principles/terms/I3> ;
                                                     rdfs:isDefinedBy <https://w3id.org/fair/fip/latest/FIP-Question-I3-MD> ;
                                                     rdfs:label "FIP Question I3-MD"@en ;
                                                     <http://www.w3.org/2004/02/skos/core#definition> "Which models, schema(s) do you use for your metadata records?"@en .


###  https://w3id.org/fair/fip/terms/FIP-Question-R1.1-D
<https://w3id.org/fair/fip/terms/FIP-Question-R1.1-D> rdf:type owl:NamedIndividual ,
                                                               <https://w3id.org/fair/fip/terms/FIP-Question> ;
                                                      <https://w3id.org/fair/fip/terms/refers-to-principle> <https://w3id.org/fair/principles/terms/R1.1> ;
                                                      rdfs:isDefinedBy <https://w3id.org/fair/fip/latest/FIP-Question-R1.1-D> ;
                                                      rdfs:label "FIP Question R1.1-D"@en ;
                                                      <http://www.w3.org/2004/02/skos/core#definition> "Which usage license do you use for your datasets?"@en .


###  https://w3id.org/fair/fip/terms/FIP-Question-R1.1-MD
<https://w3id.org/fair/fip/terms/FIP-Question-R1.1-MD> rdf:type owl:NamedIndividual ,
                                                                <https://w3id.org/fair/fip/terms/FIP-Question> ;
                                                       <https://w3id.org/fair/fip/terms/refers-to-principle> <https://w3id.org/fair/principles/terms/R1.1> ;
                                                       rdfs:isDefinedBy <https://w3id.org/fair/fip/latest/FIP-Question-R1.1-MD> ;
                                                       rdfs:label "FIP Question R1.1-MD"@en ;
                                                       <http://www.w3.org/2004/02/skos/core#definition> "Which usage license do you use for your metadata records?"@en .


###  https://w3id.org/fair/fip/terms/FIP-Question-R1.2-D
<https://w3id.org/fair/fip/terms/FIP-Question-R1.2-D> rdf:type owl:NamedIndividual ,
                                                               <https://w3id.org/fair/fip/terms/FIP-Question> ;
                                                      <https://w3id.org/fair/fip/terms/refers-to-principle> <https://w3id.org/fair/principles/terms/R1.2> ;
                                                      rdfs:isDefinedBy <https://w3id.org/fair/fip/latest/FIP-Question-R1.2-D> ;
                                                      rdfs:label "FIP Question R1.2-D"@en ;
                                                      <http://www.w3.org/2004/02/skos/core#definition> "Which metadata schemas do you use for describing the provenance of your datasets?"@en .


###  https://w3id.org/fair/fip/terms/FIP-Question-R1.2-MD
<https://w3id.org/fair/fip/terms/FIP-Question-R1.2-MD> rdf:type owl:NamedIndividual ,
                                                                <https://w3id.org/fair/fip/terms/FIP-Question> ;
                                                       <https://w3id.org/fair/fip/terms/refers-to-principle> <https://w3id.org/fair/principles/terms/R1.2> ;
                                                       rdfs:isDefinedBy <https://w3id.org/fair/fip/latest/FIP-Question-R1.2-MD> ;
                                                       rdfs:label "FIP Question R1.2-MD"@en ;
                                                       <http://www.w3.org/2004/02/skos/core#definition> "Which metadata schemas do you use for describing the provenance of your metadata records?"@en .


###  https://w3id.org/fair/principles/terms/A1.1
<https://w3id.org/fair/principles/terms/A1.1> rdf:type owl:NamedIndividual ;
                                              rdfs:label "A1.1" .


###  https://w3id.org/fair/principles/terms/A1.2
<https://w3id.org/fair/principles/terms/A1.2> rdf:type owl:NamedIndividual ;
                                              rdfs:label "A1.2" .


###  https://w3id.org/fair/principles/terms/A2
<https://w3id.org/fair/principles/terms/A2> rdf:type owl:NamedIndividual ;
                                            rdfs:label "A2" .


###  https://w3id.org/fair/principles/terms/F1
<https://w3id.org/fair/principles/terms/F1> rdf:type owl:NamedIndividual ;
                                            rdfs:label "F1" .


###  https://w3id.org/fair/principles/terms/F2
<https://w3id.org/fair/principles/terms/F2> rdf:type owl:NamedIndividual ;
                                            rdfs:label "F2" .


###  https://w3id.org/fair/principles/terms/F3
<https://w3id.org/fair/principles/terms/F3> rdf:type owl:NamedIndividual ;
                                            rdfs:label "F3" .


###  https://w3id.org/fair/principles/terms/F4
<https://w3id.org/fair/principles/terms/F4> rdf:type owl:NamedIndividual ;
                                            rdfs:label "F4" .


###  https://w3id.org/fair/principles/terms/I1
<https://w3id.org/fair/principles/terms/I1> rdf:type owl:NamedIndividual ;
                                            rdfs:label "I1" .


###  https://w3id.org/fair/principles/terms/I2
<https://w3id.org/fair/principles/terms/I2> rdf:type owl:NamedIndividual ;
                                            rdfs:label "I2" .


###  https://w3id.org/fair/principles/terms/I3
<https://w3id.org/fair/principles/terms/I3> rdf:type owl:NamedIndividual ;
                                            rdfs:label "I3" .


###  https://w3id.org/fair/principles/terms/R1.1
<https://w3id.org/fair/principles/terms/R1.1> rdf:type owl:NamedIndividual ;
                                              rdfs:label "R1.1" .


###  https://w3id.org/fair/principles/terms/R1.2
<https://w3id.org/fair/principles/terms/R1.2> rdf:type owl:NamedIndividual ;
                                              rdfs:label "R1.2" .


###  Generated by the OWL API (version 5.1.11) https://github.com/owlcs/owlapi/
